# 1

$f(x,y,z)=(\sin xy)e^{-z^2}$
$P=(1,\pi,0)$

$f_x'(x,y,z)=y(\cos xy)e^{-z^2}$
$f_y'(x,y,z)=x(\cos xy)e^{-z^2}$
$f_z'(x,y,z)=-2z(\sin xy)e^{-z^2}$

$\nabla f=\langle y(\cos xy)e^{-z^2},x(\cos xy)e^{-z^2},-2z(\sin xy)e^{-z^2}\rangle$
$\nabla f(P)=\langle-\pi,-1,0\rangle$
$\square$

You would need to go in the $\langle-\pi,-1,0\rangle$ direction as $\nabla f$ represents the direction of steepest ascent.

# 2

$x^2+2y^2+3z^2=10$
$P=(0,\sqrt2,\sqrt2)$

$\begin{cases}2x+6zf_x'=0\\4y+6zf_y'=0\end{cases}$
$\begin{cases}f_x'=-x/3z\\f_y'=-2y/3z\end{cases}$

$L_{(a,b,c)}(x,y)=c-\frac{a}{3c}(x-a)-\frac{2b}{3c}(y-b)$
$L_{(0,\sqrt2,\sqrt2)}(x,y)=\sqrt2-\frac{2}{3}(y-\sqrt2)$
$=-\frac{2}{3}y+\frac{5\sqrt2}{3}$
$\square$