---
date created: 2023-09-10 19:18
date updated: 2023-09-10 19:44
---

# 3

$\langle0,1,1\rangle\cdot\langle-7,41,-39\rangle$
$=0+41+-39$
$=\fbox{2}$

# 13

$\vec{a}=\langle1,1,1\rangle$
$\vec{b}=\langle1,-2,-2\rangle$
$\vec{a}\cdot\vec{b}=\|\vec{a}\|\|\vec{b}\|\cos(\theta)$

$\langle1,1,1\rangle\cdot\langle1,-2,-2\rangle$
$=1-2-2$
$=-3$

$\|\vec{a}\|=\sqrt3$
$\|\vec{b}\|=3$

$\cos\theta=\frac{-\sqrt3}{3}$
$\theta=2.19$

$\theta>\pi/2$
$\therefore\theta\text{ is obtuse }\fbox{}$

# 19

$\vec{a}=\langle0,3,1\rangle$
$\vec{b}=\langle4,0,0\rangle$
$\vec{a}\cdot\vec{b}=\|\vec{a}\|\|\vec{b}\|\cos(\theta)$

$\langle0,3,1\rangle\cdot\langle4,0,0\rangle$
$=0$

$\|\vec{a}\|=\sqrt{10}$
$\|\vec{b}\|=2$

$\cos\theta=0$

# 27

$\vec{a}=\langle0,1,1\rangle$
$\vec{b}=\langle1,-1,0\rangle$
$\vec{a}\cdot\vec{b}=\|\vec{a}\|\|\vec{b}\|\cos(\theta)$

$\langle0,1,1\rangle\cdot\langle1,-1,0\rangle$
$=-1$

$\|\vec{a}\|=\sqrt2$
$\|\vec{b}\|=\sqrt2$

$\cos\theta=\frac{-1}{2}$
$\theta=\fbox{2.09}$

# 43

$2\vec{u}\cdot(3\vec{u}-\vec{v})$
$=6(\vec{u}\cdot\vec{u})-2(\vec{u}\cdot{\vec{v}})$
$=6\|\vec{u}\|^2-2(2)$
$=6-4$
$=\fbox{2}$
