---
date created: 2023-09-28 11:19
date updated: 2023-09-28 23:19
---

# 9

$\vec r(t)=\langle t,t^3,t^2+1\rangle$
If $\vec r$ intersects then $xy$ plane, its $z$ value must be $0$ somewhere.

$t^2+1=0$
$t=i$

$\vec r$ does not intersect the $xy$ plane unless $t$ is a complex variable and can have the value of $i$
$\square$

# 11

$\vec r(t)=\langle1-\cos(2t),t+\sin t,t^2\rangle$

$\vec r$ will intersect the $yz$ plane if its $x$ value equals $0$ at some point.

$1-\cos(2t)=0$
$1=\cos(2t)$
$t=R\pi,\quad \text{where }R\in\mathbb I$

This proves that $\vec r$ intersects the $yz$ plane in infinitely many places
$\square$

In order for $\vec r$ to never cross the $yz$ plane, it must have all values on one side of it, or disconnected values on both sides of it.

However, we can see that:

$-1\le\cos(x)\le1$
$0\le1-\cos(2t)\le2$

Where the domain of the x value of $\vec r$ is $[0,2]$, and therefore never crosses the $yz$ plane.
$\square$

# 19

$\vec r(t)=(9\cos t)\hat i+(9\sin t)\hat j$

Since $\vec r$ has no $\hat k$ component, its $z$ value is always $0$, and it must lie on the $xy$ plane.
$\square$

We can convert $\hat i\hat j\hat k$ notation back into $xyz$ notation

$\vec r(t)=\cases{x=9\cos t\\y=9\sin t}$
$\vec r(t)=\cases{x^2=9^2\cos^2 t\\y^2=9^2\sin^2 t}$
$\vec r(t)=\cases{x^2+y^2=9^2(\sin^2t+\cos^2t)}$
$\vec r(t)=\cases{x^2+y^2=9^2}$

Where $(x-x_0)^2+(y-y_0)^2=r^2$ is the formula for a circle
Meaning
$\cases{x_0=0\\y_0=0\\r=9}$

Therefore the center of the circle is $(0,0)$ and has a radius of $9$
$\square$

# 31

## a

$C=\cases{x^2+y^2=z^2\\y=z^2}$

$C(t)=\cases{x^2+y^2=t^2\\y=t^2}$
$C(t)=\cases{x^2+y^2=y\\z=t\\y=t^2}$
$C(t)=\cases{x=\pm\sqrt{y-y^2}\\z=t\\y=t^2}$
$C(t)=\cases{x=\pm\sqrt{t^2-t^4}\\z=t\\y=t^2}$
$C(t)=\langle\pm\sqrt{t^2-t^4},t^2,t\rangle$

Or

$C(t)=\begin{cases}\langle\sqrt{t^2-t^4},t^2,t\rangle&x\ge0\\\langle-\sqrt{t^2-t^4},t^2,t\rangle&x\le0\end{cases}$
$\square$

## b

The projection of $C(t)$ onto the $xy$ plane would look like the curve with all $z$ values set to $0$

$C(t)=\langle\pm\sqrt{t^2-t^4},t^2,0\rangle$
Let $\tilde t=t^2$
$C(t)=\langle\pm\sqrt{\tilde t-\tilde t^2},t,0\rangle$
$C(t)=\begin{cases}x=\pm\sqrt{\tilde t-\tilde t^2}\\y=\tilde t\end{cases}$
$C(t)=\begin{cases}x^2=\tilde t-\tilde t^2\\y^2=\tilde t^2\end{cases}$
$C(t)=\begin{cases}x^2+y^2=\tilde t\end{cases}$
$C(t)=\begin{cases}x^2+y^2=t^2\end{cases}$
$C(t)=\begin{cases}x^2+y^2=y\end{cases}$
$C(t)=\begin{cases}x^2+y^2-y=0\end{cases}$
$C(t)=\begin{cases}x^2+(y-0.5)^2-0.25=0\end{cases}$
$C(t)=\begin{cases}x^2+(y-0.5)^2=0.5^2\end{cases}$

Where $(x-x_0)^2+(y-y_0)^2=r^2$ is the formula for a circle

Meaning:

$\cases{x_0=0\\y_0=0.5\\r=0.5}$

The projection of $C(t)$ onto the $xy$ plane looks like a circle centered at $(0,0.5)$ with a radius of $0.5$
$\square$

## c

$C(t)=\cases{x=\pm\sqrt{t^2-t^4}\\z=t\\y=t^2}$
$C(t)=\cases{x^2=t^2-t^4\\y^2=t^4\\z^2=t^2}$
$C(t)=\cases{x^2=t^2-t^4\\y^2=t^4\\z^2=t^2\\(y-1)^2=y^2-2y+1}$
$C(t)=\cases{x^2=t^2-t^4\\y^2=t^4\\z^2=t^2\\(y-1)^2=t^4-2t^2+1}$
$C(t)=\cases{x^2+(y-1)^2+z^2=t^2-t^4+t^4-2t^2+1+t^2}$
$C(t)=\cases{x^2+(y-1)^2+z^2=1}$

Where $(x-x_0)^2+(y-y_0)^2+(z-z_0)^2=r^2$ is the formula for a sphere

Meaning:

$\cases{x_0=0\\y_0=1\\z_0=0\\r=1}$

Meaning $C(t)$ lies on the sphere centered on $(0,1,0)$ with a radius of $1$
$\square$
