---
date created: 2023-09-17 23:07
date updated: 2023-09-18 02:41
---

# 1.1

## a

The sample space would be a sequence of four digits, where each digit can either be H or T

## b

Any natural number

## c

Any real number above 0

## d

Any real number above 0

## e

Any rational number between 0 and 1

# 1.4

## a

$P(A\cup B)$
$=P(A)+P(B)-P(A\cap B)$

## b

$P((A\setminus B)\cup(B\setminus A))$
$=P(A\setminus B)+P(B\setminus A)$
$=P(A\cap B^C)+P(B\cap A^C)$
$=P(A)-P(A\cap B)+P(B)-P(A\cap B)$
$=P(A)+P(B)-2P(A\cap B)$

## c

$P(A\cup B)$
$=P(A)+P(B)-P(A\cap B)$

## d

$P((A\setminus B)\cup(B\setminus A))$
$=P(A\setminus B)+P(B\setminus A)$
$=P(A\cap B^C)+P(B\cap A^C)$
$=P(A)-P(A\cap B)+P(B)-P(A\cap B)$
$=P(A)+P(B)-2P(A\cap B)$

# 1

Let $(S, B, P)$ be a probability model and let $A, B\in B$. Using only the Kolmogorov axioms and Theorem 1 on slide 9 in Lecture 2.1 show the following:

1. $P(A) = P (A \cap B) + P (A \cap B^C)$
2. $P(A\setminus B)=P(A)-P(A\cap B)$
3. $P(A\cup B)=P(A)+P(B)-P(A\cap B)$
4. If $A\subseteq B$ then $P(A)\le P(B)$

You may prove the four parts in any order you like. Just make sure you don’t go in a circle, e.g. use (b) to prove (a) and then use (a) to prove (b)

## a

$P(A) = P (A \cap B) + P (A \cap B^C)$
Since $B$ and $B^C$ are disjoint, $A\cap B$ and $A\cap B^C$ are also disjoint
Define $B_1^*=B$ and $B_2^*=B^C$
$P(A\cap B)+P(A\cap B^C)$
$=P(A\cap B_1^*)+P(A\cap B_2^*)$
$=\sum\limits_{i=1}^2 P(A\cap B_i^*)$
$=P(\bigcup\limits_{i=1}^2 A\cap B_i^*)$
$=P((A\cap B_1^*)\cup((A\cap B_2^*)))$
$=P((A\cap B)\cup(A\cap B^C))$
$=P(A\cap(B\cup B^C))$
$=P(A\cap\mathbb{U})$
$=P(A)$
$\square$

## b

$P(A\setminus B)=P(A)-P(A\cap B)$

$A\setminus B=\{x:x\in A : x\notin B\}$
$=A\cap B^C$

$P(A) = P (A \cap B) + P (A \cap B^C)$
$=P(A\cap B)+P(A\setminus B)$

$P(A\setminus B)=P(A)-P(A\cap B)$
$\square$
## c

$P(A\cup B)=P(A)+P(B)-P(A\cap B)$

$P(A\cup B)=P((A\cup B)\cap B)+P((A\cup B)\cap B^C)$
$=P(B)+P((A\cap B^C)\cup (B\cap B^C))$
$=P(B)+P(A\cap B^C)$
$=P(B)+P(A\cap B^C)+P(A\cap B)-P(A\cap B)$
$=P(B)+P(A)-P(A\cap B)$
$\square$

## d

If $A\subseteq B$ then $P(A)\le P(B)$

If $A=B$ then $P(A)=P(B)$

If $A\subset B$ then $x\in A\implies x\in B$
$A=\{x:x\in A\}$
$A=\{x:x\in A:x\in B\}$
$A\cap B=\{x:x\in A:x\in B\}$
$A\cap B=A$
$P(A\cap B)=P(A)$

$P(B)=P(A\cap B)+P(A^C\cap B)$
$=P(A)+P(A^C\cap B)$

$P(A^C\cap B)>0$

$P(B)>P(A)$

# 2

Draw Venn diagrams to illustrate DeMorgan’s laws
$(A\cup B)^C=A^C\cap B^C$ and $(A\cap B)^C=A^C\cup B^C$

![[2a.svg]]
![[2b.svg]]