# 4.43

## a

$\text{Cov}(X_1+X_2,X_2+X_3)=E((X_1+X_2)(X_2+X_3))-E(X_1+X_2)E(X_2+X_3)$
$=E(X_1X_2)+E(X_1X_3)+E(X_2X_2)+E(X_2X_3)-(2\mu)(2\mu)$
$=+E(X_1)E(X_2)+E(X_1)E(X_3)+\text{Cov}(X_2,X_2)+E(X_2)E(X_3)+E(X_2)E(X_3)-4\mu^2$
$=\mu^2+\mu^2+\sigma^2+\mu^2+\mu^2-4\mu^2$
$=\sigma^2$

## b

$\text{Cov}(X_1+X_2,X_1-X_2)=E((X_1+X_2)(X_1-X_2))-E(X_1+X_2)E(X_1-X_2)$
$=E(X_1X_1-X_1X_2+X_2X_1-X_2X_2)$
$=E(X_1X_1)-E(X_2X_2)$
$=E(X_1X_1)-E(X_2X_2)$
$=\sigma^2-\sigma^2$
$=0$

# 4.45

## a

$f(x,y)=\frac{1}{2\pi\sigma_X\sigma_Y\sqrt{1-\rho^2}}\exp\left( -\frac{1}{2(1-\rho^2)}\left( \left( \frac{x-\mu_X}{\sigma_X} \right)^2 -2\rho \left( \frac{x-\mu_x}{\sigma_X} \right)\left( \frac{y-\mu_Y}{\sigma_Y} \right) + \left( \frac{y-\mu_Y}{\sigma_Y} \right)^2 \right) \right)$

$z_X=\frac{x-\mu_X}{\sigma_X}$
$z_Y=\frac{y-\mu_Y}{\sigma_Y}$

$f(x,y)=\frac{1}{2\pi\sigma_X\sigma_Y\sqrt{1-\rho^2}}\exp\left( -\frac{z_X^2 -2\rho z_Xz_Y + z_Y^2}{2(1-\rho^2)}\right)$
$f(x,y)=\frac{1}{2\pi\sigma_X\sigma_Y\sqrt{1-\rho^2}}\exp\left( -\frac{(z_X -\rho z_Y)^2 + z_Y^2(1- \rho^2) }{2(1-\rho^2)}\right)$
$f(x,y)=\frac{1}{\sqrt{2\pi}\sigma_Y\sqrt{1-\rho^2}}\exp\left( -\frac{z_Y^2}{2} \right) \frac{1}{\sqrt{2\pi}\sigma_X}\exp\left( -\frac{(z_X -\rho z_Y)^2}{2(1-\rho^2)}\right)$

$f_Y(u)=\int_{-\infty}^\infty f(x,y)~dx$
$f_Y(u)=\frac{1}{\sqrt{2\pi}\sigma_Y\sqrt{1-\rho^2}}\exp\left( -\frac{z_Y^2}{2} \right) \int_{-\infty}^\infty \frac{1}{\sqrt{2\pi}\sigma_X}\exp\left( -\frac{(z_X -\rho z_Y)^2}{2(1-\rho^2)}\right)~dx$

$dx_X\sigma_X=dx$
$f_Y(u)=\frac{1}{\sqrt{2\pi}\sigma_Y}\exp\left( -\frac{z_Y^2}{2} \right) \int_{-\infty}^\infty \frac{1}{\sqrt{2\pi}\sqrt{1-\rho^2}}\exp\left( -\frac{(z_X -\rho z_Y)^2}{2\sqrt{1-\rho^2}^2}\right)~dz$
$f_Y(u)=\frac{1}{\sqrt{2\pi}\sigma_Y}\exp\left( -\frac{z_Y^2}{2} \right)$

$Y\sim\text{N}(\mu_Y,\sigma^2_Y)$

The exact same is true for $X$, just replacing $_X$ variables with $_Y$

## b

$Y|X=\frac{f_{XY}}{f_X}$

$f(x,y)=\frac{1}{2\pi\sigma_X\sigma_Y\sqrt{1-\rho^2}}\exp\left( -\frac{z_X^2 -2\rho z_Xz_Y + z_Y^2}{2(1-\rho^2)}\right)$
$f_X(x)=\frac{1}{\sigma_X\sqrt{2\pi}}\exp\left( -\frac{z_X^2}{2} \right)$

$f_{Y|X}(y|x)=\frac{1}{\sqrt{2\pi}\sigma_Y\sqrt{1-\rho^2}}\exp\left( -\frac{1}{2(1-\rho^2)}\left( \rho^2\left( \frac{x-\mu_X}{\sigma_X} \right)^2 -2\rho \left( \frac{x-\mu_x}{\sigma_X} \right)\left( \frac{y-\mu_Y}{\sigma_Y} \right) + \left( \frac{y-\mu_Y}{\sigma_Y} \right)^2 \right)\right)$
$f_{Y|X}(y|x)=\frac{1}{\sqrt{2\pi}\sigma_Y\sqrt{1-\rho^2}}\exp\left( -\frac{1}{2(1-\rho^2)}\left(\left(\left( \frac{y-\mu_Y}{\sigma_Y} \right)-\rho\left( \frac{x-\mu_x}{\sigma_X} \right)\right)^2 \right)\right)$
$f_{Y|X}(y|x)=\frac{1}{\sqrt{2\pi}\sigma_Y\sqrt{1-\rho^2}}\exp\left( -\frac{1}{2\sigma^2_Y(1-\rho^2)}\left(y-\left(\mu_Y +\frac{\rho\sigma_Y(x-\mu_x)}{\sigma_X}\right) \right)^2 \right)$

$\sim\text{N}(\mu_Y +\rho(\sigma_Y/\sigma_X)(x-\mu_x),\sigma_Y^2(1-\rho^2))$

## c

$U=aX+bY$
$V=Y$

$X=\frac{U-bV}{a}$
$Y=V$

$J=\begin{vmatrix} \frac{1}{a} & -\frac{b}{a} \\ 0 & 1\end{vmatrix}= \frac{1}{a}$

$z_X= \frac{\frac{u-bv}{a}-\mu_X}{\sigma_X}=\frac{u-(bv+a\mu_X)}{a\sigma_X}$

$f(x,y)=\frac{1}{2\pi\sigma_X\sigma_Y\sqrt{1-\rho^2}}\exp\left( -\frac{z_X^2 -2\rho z_Xz_Y + z_Y^2}{2(1-\rho^2)}\right)$
$f_{UV}(u,v)=\frac{1}{2a\pi\sigma_X\sigma_Y\sqrt{1-\rho^2}}\exp\left( -\frac{(\frac{u-(bv+a\mu_X)}{a\sigma_X})^2 -2\rho (\frac{u-(bv+a\mu_X)}{a\sigma_X})z_V + z_V^2}{2(1-\rho^2)}\right)$

Let
$A=(\frac{u-(bv+a\mu_X)}{a\sigma_X})^2 -2\rho (\frac{u-(bv+a\mu_X)}{a\sigma_X})z_V + z_V^2$
$=\left( \frac{u-(bv+a\mu_X)}{a\sigma_X} \right)^2 -2\rho \left( \frac{u-(bv+a\mu_X)}{a\sigma_X} \right)\left( \frac{v-\mu_Y}{\sigma_Y} \right) + \left( \frac{v-\mu_Y}{\sigma_Y} \right)^2$
$=\frac{1}{a^2\sigma_X^2\sigma_Y^2}(\sigma_Y^2(u^2-2buv-2au\mu_X+b^2v^2+2bva\mu_X+a^2\mu_X^2)-2\rho a\sigma_X\sigma_Y \left(uv-u\mu_Y-bv^2-av\mu_X+\mu_Ybv+\mu_Ya\mu_X\right)+a^2\sigma_X^2(v^2-2v\mu_Y+\mu_Y^2)$

$=(\sigma_Y^2b^2+2\rho ab\sigma_X\sigma_Y+a^2\sigma_X^2)v^2+(-2\sigma_Y^2bu+2\sigma_Y^2ab\mu_X-2\rho a\sigma_X\sigma_Yu+2\rho a\sigma_X\sigma_Ya\mu_X-2\rho a\sigma_X\sigma_Y\mu_Yb-2a^2\sigma_X^2\mu_Y)v$
$+\sigma_Y^2(u^2-2au\mu_X+a^2\mu_X^2)-2\rho a\sigma_X\sigma_Y(-u\mu_Y+\mu_Ya\mu_X)+a^2\sigma_X^2\mu_Y^2$

# 5.3

$Y_i=\text{Bernoulli}(1-F(\mu))$
$\sum\limits_{i=1}^nY_i\sim\text{Binomial}(n, 1-F(\mu))$

# 5.5

$\bar X= \frac{1}{n}(X_1+...+X_n)$
$\bar X= \frac{1}{n}Y$

$f_{\bar X}=nf_Y(nx)$
$f_{\bar X}=nf_{X_1+...+X_n}(nx)$

# 5.6

## a

$U=X+Y$
$V=Y$

$X=U-V$
$Y=V$

$J=1$

$f_{UV}(u,v)=f_{XY}(u-v,v)$
$f_U(u)=\int\limits_{-\infty}^\infty f_X(u-v)f_Y(v)~dv$

## b

$U=XY$
$V=Y$

$X=\frac{U}{V}$
$Y=V$

$J=\frac{1}{V}$

$f_{UV}(u,v)=|\frac{1}{v}|f_{XY}\left( \frac{u}{v},v \right)$
$f_U(u)=\int\limits_{-\infty}^\infty |\frac{1}{v}|f_X\left(\frac{u}{v} \right)f_Y\left(v\right)~ dv$

## c

$U=\frac{X}{Y}$
$V=Y$

$X=UV$
$Y=V$

$J=V$

$f_{UV}(u,v)=|v|f_{XY}(uv,v)$
$f_U(u)=|v|f_X(uv)f_Y(v)~ dv$
