---
date created: 2023-09-03 19:30
date updated: 2023-09-03 19:57
---

# 13

A and C, $\langle4, 8, 12\rangle\|\langle2, 4, 6\rangle\|\langle-7, -14, -21\rangle$

# 15

$\vec{AB}=\langle-3, -2, -1\rangle$
$\vec{PQ}=\langle-5, -3, -6\rangle$
No, $\vec{AB}\neq\vec{PQ}$

# 43

$\vec{v}(t)=\langle1, 2, -8\rangle+t\langle2, 1, 3\rangle$

# 45

$\vec{v}(t)=\langle4, 0, 8\rangle+t\langle7, 0, 4\rangle$

# 51

$\vec{v}(t)=t\langle0, 0, 1\rangle$

# 57

$\vec{r_1}(t_1)=\langle3, -1, 4\rangle+t_1\langle8, 12, -6\rangle$
$\vec{r_2}(t_2)=\langle11, 11, -2\rangle+t_2\langle4, 6, -3\rangle$

Let $t_2=2t_1-2$

$\vec{r_2}(t_2)=\langle11, 11, -2\rangle+(2t_1-2)\langle4, 6, -3\rangle$
$\vec{r_2}(t_2)=\langle11, 11, -2\rangle+2t_1\langle4, 6, -3\rangle-\langle8, 12, -6\rangle$
$\vec{r_2}(t_2)=\langle3, -1, 4\rangle+t_1\langle8, 12, -6\rangle$

$\therefore \vec{r_1}(t)=\vec{r_2}(2t-2)$
And do represent the same line.
# 61

$\vec{r_1}(t)=\langle-1, 2, 2\rangle+t\langle4, -2, 1\rangle$
$\vec{r_2}(s)=\langle0, 1, 1\rangle+s\langle2, 0, 1\rangle$
$\langle-1, 2, 2\rangle+t\langle4, -2, 1\rangle=\langle0, 1, 1\rangle+s\langle2, 0, 1\rangle$

$-1+4t=2s$
$2-2t=1$
$2+t=1+s$

$$

# 65
