---
date created: 2023-09-10 19:49
date updated: 2023-09-10 19:49
---

# 9

$\vec{a}=\langle1,2,1\rangle$
$\vec{b}=\langle3,1,1\rangle$

$\langle1,2,1\rangle\times\langle3,1,1\rangle$
$=\begin{vmatrix}\hat{i}&\hat{j}&\hat{k}\\1&2&1\\3&1&1\end{vmatrix}$

$=\langle1,2,-5\rangle\fbox{}$

# 17

$(\hat{i}-3\hat{j}+2\hat{k})\times(\hat{j}-\hat{k})$
$=\langle1,-3,2\rangle\times\langle0,1,-1\rangle$
$=\begin{vmatrix}\hat{i}&\hat{j}&\hat{k}\\1&-3&2\\0&1&-1\end{vmatrix}$
$=\langle1,1,1\rangle$

$(\hat{i}-3\hat{j}+2\hat{k})\times(\hat{j}-\hat{k})$
$=\hat{k}+\hat{j}+3\hat{i}-2\hat{i}$
$=\hat{i}+\hat{j}+\hat{k}$
$=\langle1,1,1\rangle$

# 23

$(\vec{u}-2\vec{v})\times(\vec{u}+2\vec{v})$
$=2(\vec{u}\times\vec{v})-2(\vec{v}\times\vec{u})$

# 41

# 47
