---
date created: 2023-09-28 23:19
---

# 1

$\lim\limits_{x\rightarrow3}\langle t^2,4t,1/t\rangle$

$t^2,4t,1/t$ are all continuous at 3, so we can just evaluate at 3

$\langle 9,12,1/3\rangle$
$\square$

# 5

$\lim\limits_{h\rightarrow0}(\vec r(t+h)-\vec r(t))/h$
$\vec r(t)=\langle t^{-1},\sin t,4\rangle$

$\lim\limits_{h\rightarrow0}(\langle (t+h)^{-1},\sin (t+h),4\rangle-\langle t^{-1},\sin t,4\rangle)/h$
$\lim\limits_{h\rightarrow0}\langle (t+h)^{-1}-t^{-1},\sin (t+h)-\sin t,4-4\rangle/h$
$\lim\limits_{h\rightarrow0}\langle (-1)/(t(t+h)),(\sin (t+h)-\sin t)/h,0\rangle$
$\lim\limits_{h\rightarrow0}\langle -1/(t^2+th),(\sin (t+h)-\sin t)/h,0\rangle$
$\lim\limits_{h\rightarrow0}\langle -1/(t^2+th),(\sin t\cos h+\cos t\sin h-\sin t)/h,0\rangle$
$\lim\limits_{h\rightarrow0}\langle -1/(t^2+th),(\sin t(\cos h-1)+\cos t\sin h)/h,0\rangle$
$\lim\limits_{h\rightarrow0}\langle -1/(t^2+th),\sin t(0)+\cos t(1),0\rangle$
$\lim\limits_{h\rightarrow0}\langle -1/t^2,\cos t,0\rangle$
$\langle -1/t^2,\cos t,0\rangle$
$\square$

# 7

$\vec r(t)=\langle t,t^2,t^3\rangle$
$\vec r'(t)=\langle (t)',(t^2)',(t^3)'\rangle$
$\vec r'(t)=\langle 1,2t,3t^2\rangle$
$\square$

# 17

$\vec r(t)=\langle t-\sin t,1-\cos t\rangle$
Parallel to $\langle\sqrt3,1\rangle$
$\vec r'(t)=C\langle\sqrt3,1\rangle$

$\vec r'(t)=\langle1-\cos t,\sin t\rangle$
$\langle1-\cos t,\sin t\rangle=\langle C\sqrt 3,C\rangle$
$(1-\cos t)/\sin t=\sqrt3$
$t=2\pi/3$
$\square$

# 25

$\vec r(t)=\langle t^2,1-t\rangle\quad g(t)=e^t$
$\frac{d}{dx}\vec r(g(t))=\vec r'(g(t))g'(t)$

$\vec r'(t)=\langle2t,-1\rangle$
$g'(t)=e^t$

$\frac{d}{dx}\vec rg(t))=\langle 2e^t,-1\rangle e^t$
$\frac{d}{dx}\vec rg(t))=\langle 2e^{2t},-e^t\rangle$
$\square$

# 39

$\vec r(t)=\langle t,1,1\rangle$
$\|\vec r'(t)\|=\|\langle1,0,0\rangle\|=1$
$\|\vec r(t)\|'=\sqrt{t^2+2}'=t/\sqrt{t^2+2}$

1 does not always equal $t/\sqrt {t^2+2}$
$\square$
