---
date created: 2023-10-10 10:06
---

# 13

NW

# 19

$z=\frac{x}{y}$
$\frac{\partial}{\partial x}=\frac{1}{y}$
$\frac{\partial}{\partial y}=\frac{-x}{y^2}$
$\square$

# 25

$z=\cos\frac{1-x}{y}$
$\frac{\partial}{\partial x}=\frac{1}{y}\sin\frac{1-x}{y}$
$\frac{\partial}{\partial y}=\frac{x-1}{y^2}\sin\frac{1-x}{y}$
$\square$

# 33

$z=e^{-x^2-y^2}$
$\frac{\partial}{\partial x}=-2xe^{-x^2-y^2}$
$\frac{\partial}{\partial y}=-2ye^{-x^2-y^2}$
$\square$

# 41

$Q=\frac{L}{M}e^{-Lt/M}$
$\frac{\partial}{\partial L}=(\frac{-Lt}{M^2}+\frac{1}{M})e^{-Lt/M}$
$\frac{\partial}{\partial M}=(\frac{-L}{M^2}+\frac{L^2t}{M^3})e^{-Lt/M}$
$=\frac{L(Lt-M)}{M^3}e^{-Lt/M}$
$\frac{\partial}{\partial M}=\frac{-L^2}{M^2}e^{-Lt/M}$
$\square$

# 57

$f(x,y)=x\ln(y^2)$
$\frac{\partial}{\partial y}=\frac{2x}{y}$
$\frac{\partial^2}{\partial^2 y}=\frac{-2x}{y^2}$
$\frac{\partial^2}{\partial^2 y}(2,3)=\frac{-4}{9}$

# 61

$f(u,v)=\cos(u+v^2)$
$\frac{\partial}{\partial u}=-\sin(u+v^2)$
$\frac{\partial^2}{\partial^2 u}=-\sin(u+v^2)$
