# 3

$P=(-1,2)$
$f(x,y)=xy^2+x^3y^2$
$f'_x(x,y)=y^2+3x^2y^2$
$f'_y(x,y)=2xy+2x^3y$

$f_x'(P)=16$
$f_y'(P)=-8$
$f(P)=-8$

$A=-8+16(x+1)-8(y-2)$
$A=16x-8y+24$
$\square$

# 5

$P=(4,1)$
$f(x,y)=x^2+y^{-2}$
$f_x'(x,y)=2x$
$f_y'(x,y)=-2y^{-3}$

$f_x'(P)=8$
$f_y'(P)=-2$
$f(P)=17$

$A=17+8(x-4)-2(y-1)$
$A=8x-2y-13$
$\square$

# 7

$P=(2,1)$
$F(r,s)=r^2s^{-1/2}+s^{-3}$
$F_r'(r,s)=2rs^{-1/2}$
$F_s'(r,s)=-0.5r^2s^{-3/2}-3s^{-4}$

$F_r'(P)=4$
$F_s'(P)=-5$
$F(P)=5$

$A=5+4(r-2)-5(s-1)$
$A=4r-5s+2$
$\square$

# 13

$f(x,y)=3x^2-xy-y^2$
$f_x'(x,y)=6x-y$
$f_y'(x,y)=-x-2y$

$\begin{cases}6x-y=0\\-x-2y=0\end{cases}$
$\begin{cases}6x-y=0\\-x-12x=0\end{cases}$
$\begin{cases}y=0\\x=0\end{cases}$

$P=(0,0)$
$\square$

# 15

$P=(2,1)$
$f(x,y)=x^2y^3$
$f_x'(x,y)=2xy^3$
$f_y'(x,y)=3x^2y^2$

$L_{(a,b)}(x,y)=a^2b^3+2ab^3(x-a)+3a^2b^2(y-b)$
$L_P(x,y)=4+4(x-2)+12(y-1)$
$L_P(x,y)=4x+12y-16$
$\square$

$L_P(2.01,1.02)=4.28$
$L_P(1.97,1.01)=4$
$\square$

# 23

$f(2,4)=5$
$f_x'(2,4)=0.3$
$f_y'(2,4)=-0.2$

$L_{(2,4)}(x,y)=5+0.3(x-2)-0.2(y-4)$
$L_{(2,4)}(x,y)=0.3x-0.2y+5.2$
$\square$

$L_{(2,4)}(2.1,3.8)=5.07$
$\square$

# 43

## a

$f(x,y)=5x+4y^2$
$f_x'(x,y)=5$
$f_y'(x,y)=8y$

$L_{(a,b)}(x,y)=6a+4b^2+5(x-a)+8b(y-b)$
$L_{(2,1)}(x,y)=14+5(x-2)+8(y-1)$
$L_{(2,1)}(x,y)=5x+8y-4$
$\square$

$L(x,y)+4(y-1)^2=5x+8y-4+4y^2-8y+4$
$=5x+4y^2$
$=f(x,y)$
$\square$

## b

$\frac{4(y-1)^2}{\sqrt{(x-2)^2+(y-1)^2}}$

Since $(x-2)^2$ and $(y-1)^2$ are positive, the denominator is also positive.
Since $(y-1)^2$ is positive, so is the numerator and thus the whole fraction $\ge0$

$=4\sqrt{\frac{(y-1)^4}{(x-2)^2+(y-1)^2}}$
$=4\sqrt{\frac{((x-2)^2-(y-1)^2)(y-1)^4}{((x-2)^2+(y-1)^2)((x-2)^2-(y-1)^2)}}$
$=4\sqrt{\frac{((x-2)^2-(y-1)^2)(y-1)^4}{(x-2)^4-(y-1)^4}}$
