---
date created: 2023-10-19 22:04
---

# 9

$f(x,y)=3x-7y$
$\vec r(t)=\langle\cos t,\sin t\rangle$
$t=0$

$\frac{d}{dt}f(\vec r(t))=\nabla f(\vec r(t))\cdot\vec r'(t)$

$\nabla f(\vec r(t))=\langle3,-7\rangle$
$\vec r'(t)=\langle-\sin t,\cos t\rangle$

$\nabla f(\vec r(t))\cdot \vec r'(t)=-3\sin t-7\cos t$
$\nabla f(\vec r(0))\cdot \vec r'(0)=-7$
$\square$

# 11

$f(x,y)=x^2-3xy$
$\vec r(t)=\langle\cos t,\sin t\rangle$
$t=0$

$\frac{d}{dt}f(\vec r(t))=\nabla f(\vec r(t))\cdot\vec r'(t)$

$\nabla f(\vec r(t))=\langle2\cos t-3\sin t,-3\cos t\rangle$
$\vec r'(t)=\langle-\sin t,\cos t\rangle$

$\nabla f(\vec r(0))\cdot \vec r'(0)=0+-3$
$=-3$
$\square$

# 15

$f(x,y)=x-xy$
$\vec r(t)=\langle t^2,t^2-4t\rangle$
$t=4$

$\frac{d}{dt}f(\vec r(t))=\nabla f(\vec r(t))\cdot\vec r'(t)$

$\nabla f(\vec r(t))=\langle1-(t^2-4t),-(t^2)\rangle$
$\vec r'(t)=\langle2t,2t-4\rangle$

$\nabla f(\vec r(4))\cdot \vec r'(4)=1*8+-16*4$
$=-56$
$\square$

# 17

$f(x,y)=\ln x+\ln y$
$\vec r(t)=\langle\cos t,t^2\rangle$
$t=\frac{\pi}{4}$

$\nabla f(\vec r(0))\cdot \vec r'(0)=0+-3$

$\nabla f(\vec r(t))=\langle\frac{1}{\cos t},\frac{1}{t^2}\rangle$
$\vec r'(t)=\langle-\sin t,2t\rangle$

$\nabla f(\vec r(\frac{\pi}{4}))\cdot \vec r'(\frac{\pi}{4})=-1+\frac{8}{\pi}$
$=\frac{8}{\pi}-1$
$\square$

# 21

$f(x,y)=x^2+y^3$
$\vec v=\langle 4,3\rangle$
$P=(1,2)$

$\nabla f(P)=\langle2,12\rangle$
$\nabla f(P)\cdot\vec v/\|\vec v\|=8/5+36/5$
$=44/5=8.8$

# 27

$f(x,y)=\ln(x^2+y^2)$
$\vec v=3i-2j=\langle3,-2\rangle$
$P=(1,0)$

$\nabla f(P)=\langle\frac{2x}{x^2+y^2},\frac{2y}{x^2+y^2}\rangle\bigg|_{P}$
$=\langle2,0\rangle$

$\nabla f(P)\cdot\vec v/\|\vec v\|=6/\sqrt{13}$
$=\frac{6}{\sqrt{13}}=\frac{6\sqrt{13}}{13}$
$\square$

# 29

$g(x,y,z)=xe^{-yz}$
$\vec v=\langle1,1,1\rangle$
$P=(1,2,0)$

$\nabla g(P)=\langle e^{-yz},-xze^{-yz},-xye^{-yz}\rangle\bigg|_P$
$=\langle 1,0,-2\rangle$

$\nabla g(P)\cdot\vec v/\|\vec v\|=-1/\sqrt{3}$
$=\frac{-1}{\sqrt 3}=\frac{-\sqrt 3}{3}$
$\square$

# 43

$\frac{x^2}{4}+\frac{y^2}{9}+z^2=1$
$f(x,y)=z=\pm\sqrt{1-\frac{x^2}{4}-\frac{y^2}{9}}$

$\nabla f((x,y,\pm\sqrt{1-\frac{x^2}{4}-\frac{y^2}{9}}))=\langle\mp\frac{x}{4\sqrt{1-\frac{x^2}{4}-\frac{y^2}{9}}},\mp\frac{y}{9\sqrt{1-\frac{x^2}{4}-\frac{y^2}{9}}}\rangle$
Meaning the $z$ value is the opposite sign of the normal whilst $x$ and $y$ are the same

Which means the tangent plane at $(x,y)$ is
$L_{(x,y)}(a,b)=f(x,y)+\nabla f_x(a-x)+\nabla f_y(b-y)$
Making the normal to the plane
$\vec N=\langle\pm\frac{x}{4\sqrt{1-\frac{x^2}{4}-\frac{y^2}{9}}},\pm\frac{y}{9\sqrt{1-\frac{x^2}{4}-\frac{y^2}{9}}},1\rangle$

$\vec N=\langle1,1,-2\rangle$

$\begin{cases}\pm\frac{x}{4\sqrt{1-\frac{x^2}{4}-\frac{y^2}{9}}}=\frac{-1}{2}\\\pm\frac{y}{9\sqrt{1-\frac{x^2}{4}-\frac{y^2}{9}}}=\frac{-1}{2}\end{cases}$
$=\begin{cases}x=\mp2\sqrt{1-\frac{x^2}{4}-\frac{y^2}{9}}\\y=\mp4.5\sqrt{1-\frac{x^2}{4}-\frac{y^2}{9}}\end{cases}$
Which means that $x$ and $y$ are the same sign

$=\begin{cases}x^2=4(1-\frac{x^2}{4}-\frac{y^2}{9})\\y^2=\frac{81}{4}(1-\frac{x^2}{4}-\frac{y^2}{9})\end{cases}$
$=\begin{cases}x^2=2-\frac{2y^2}{9}\\y^2=\frac{81}{4}-\frac{81x^2}{16}-\frac{9y^2}{4}\end{cases}$
$=\begin{cases}x^2=2-\frac{2y^2}{9}\\y^2=\frac{81}{4}-\frac{81(2-\frac{2y^2}{9})}{16}-\frac{9y^2}{4}\end{cases}$
$=\begin{cases}x^2=2-\frac{2y^2}{9}\\y^2=\frac{81}{4}-\frac{81}{8}+\frac{9y^2}{8}-\frac{9y^2}{4}\end{cases}$
$=\begin{cases}x^2=2-\frac{2y^2}{9}\\y^2=\frac{81}{8}-\frac{9y^2}{8}\end{cases}$
$=\begin{cases}x^2=2-\frac{2y^2}{9}\\\frac{17}{8}y^2=\frac{81}{8}\end{cases}$
$=\begin{cases}x^2=2-\frac{2*\frac{81}{17}}{9}\\y^2=\frac{81}{17}\end{cases}$
$=\begin{cases}x^2=\frac{16}{17}\\y^2=\frac{81}{17}\end{cases}$
$(\pm\frac{4}{\sqrt{17}},\pm\frac{9}{\sqrt{17}})$
Where $x$ and $y$ are the same sign and $z$ is the opposite sign
$(\pm\frac{4}{\sqrt{17}},\pm\frac{9}{\sqrt{17}},\mp\sqrt{1-\frac{x^2}{4}-\frac{y^2}{9}})$
$(\pm\frac{4}{\sqrt{17}},\pm\frac{9}{\sqrt{17}},\mp\sqrt{1-\frac{4}{17}-\frac{9}{17}})$
$(\pm\frac{4}{\sqrt{17}},\pm\frac{9}{\sqrt{17}},\mp\sqrt{\frac{4}{17}})$
$(\pm\frac{4}{\sqrt{17}},\pm\frac{9}{\sqrt{17}},\mp\frac{2}{\sqrt{17}})$

Therefore, the Normals are $\langle1,1,-2\rangle$ at 
$(\frac{4}{\sqrt{17}},\frac{9}{\sqrt{17}},-\frac{2}{\sqrt{17}})$
and
$(-\frac{4}{\sqrt{17}},-\frac{9}{\sqrt{17}},\frac{2}{\sqrt{17}})$
$\square$

# 47

$xz+2x^2+y^2z^3=11$
$P=(2,1,1)$

$f_xx+z+4x$
