# 3

$f(x,y,z)=xy+z^2$
$x=s^2$
$y=2rs$
$z=r^2$

$f(s,r)=2rs^3+r^4$
$f_s'(s,r)=6rs^2$
$f_r'(s,r)=2s^3+4r^3$
$\square$

# 5

$g(\theta,\phi)=\tan(\theta+\phi)$
$\theta=xy$
$\phi=x+y$

$g(x,y)=\tan(xy+x+y)$
$g_x'(x,y)=\sec^2(xy+x+y)(y+1)$
$g_y'(x,y)=\sec^2(xy+x+y)(x+1)$
$\square$

# 11

$f(x,y,z)=x^3+yz^2$
$x=u^2+v$
$y=u+v^2$
$z=uv$
$(u,v)=(-1,-1)$

$f(u,v)=(u^2+v)^3+(u+v^2)(uv)^2$

$f_u'(u,v)=6u(u^2+v)^2+2(u+v^2)(uv)+(uv)^2$
$\bigg|_{(-1,-1)}=1$

$f_v'(u,v)=3(u^2+v)^2+2(u+v^2)(uv)+2v(uv)^2$
$\bigg|_{(-1,-1)}=-2$

# 15

$g(x,y)=x^2-y^2$
$x=e^u\cos v$
$y=e^u\sin v$
$(u,v)=(0,1)$

$g(u,v)=e^{2u}\cos^2v-e^{2u}\sin^2v$

$g_u'(u,v)=2e^{2u}\cos^2v-2e^{2u}\sin^2v$
$g_u'(u,v)=2e^{2u}(\cos(2v))$
$\bigg|_{(0,1)}=2\cos2$

# 25

$x=s+t$
$y=s-t$
$f(x,y)$

$\frac{\partial f}{\partial s}=\frac{\partial f}{\partial x}\frac{\partial x}{\partial s}+\frac{\partial f}{\partial y}\frac{\partial y}{\partial s}$
$\frac{\partial f}{\partial s}=\frac{\partial f}{\partial x}+\frac{\partial f}{\partial y}$

$\frac{\partial f}{\partial t}=\frac{\partial f}{\partial x}\frac{\partial x}{\partial t}+\frac{\partial f}{\partial y}\frac{\partial y}{\partial t}$
$\frac{\partial f}{\partial t}=\frac{\partial f}{\partial x}-\frac{\partial f}{\partial y}$

$=\frac{\partial f}{\partial x}+\frac{\partial f}{\partial y}$
$\frac{\partial f}{\partial t}\frac{\partial f}{\partial s}=(\frac{\partial f}{\partial x}-\frac{\partial f}{\partial y})(\frac{\partial f}{\partial x}+\frac{\partial f}{\partial y})$

$\frac{\partial f}{\partial t}\frac{\partial f}{\partial s}=(\frac{\partial f}{\partial x})^2-(\frac{\partial f}{\partial y})^2$

# 27

## a

$F(x,y,z)=xz^2+y^2z+xy-1$

## b

# 35