---
date created: 2023-10-30 14:44
---

# 7

$f(x,y)=x^2+y^2-xy+x$

$\nabla f=\langle 2x-y+1,2y-x\rangle$

$\nabla f=\langle0,0\rangle\iff(x,y)=(-2/3,-1/3)$

$H(f)=\begin{bmatrix}2&-1\\-1&2\end{bmatrix}$
$|H(f)|=5$

Since the determinant at $(-2/3,-1/3)$ is positive we can conclude it is a max/min. Since $H(f)_{xx}$ is positive, we can conclude that it is a minima.

# 9

$f(x,y)=x^3+2xy-2y^2-10x$

$\nabla f=\langle3x^2+2y-10,2x-4y\rangle$

$\nabla f=\langle0,0\rangle\iff\begin{cases}3x^2+2y-10=0\\2x-4y=0\end{cases}$
$=\begin{cases}x=2y\\6y^2+y-5=0\end{cases}$
$=\begin{cases}x=2y\\(6y-5)(y+1)=0\end{cases}$
$=\begin{cases}x=\{5/3,-2\}\\y=\{5/6,-1\}\end{cases}$
$\iff(x,y)\in\{(5/3,5/6),(-2,-1)\}$

$H(f)=\begin{bmatrix}6x&2\\2&-4\end{bmatrix}$
$|H(f)|=-24x-4$
$|H(f(5/3,5/6))|=-44$
$|H(f(-2,-1))|=44$

Since the determinant on $(5/3,5/6)$ is negative, we can conclude that it is a saddle point. Since the determinant on $(-2,-1)$ is positive and $H(f(-2,-1))_{xx}=-12$ is negative, we can conclude it is a local maximum.

# 11

$f(x,y)=4x-3x^3-2xy^2$

$\nabla f=\langle4-9x^2-2y^2,-4xy\rangle$

$\nabla f=\langle0,0\rangle\iff\begin{cases}4-9x^2-2y^2=0\\4xy=0\end{cases}$
$=\begin{cases}x=0\cup y=0\\2=y^2\cup 4/9=x^2\end{cases}$
$\iff(x,y)\in\{(0,\pm\sqrt2),(\pm2/3,0)\}$

$H(f)=\begin{bmatrix}-18x&-4y\\-4y&-4x\end{bmatrix}$
$|H(f)|=72x^2-16y^2$

$\bigg|_{(0,\pm\sqrt2)}=-32$
$\bigg|_{(\pm2/3,0)}=48$

Since the determinant on $(0,\pm\sqrt2)$ is negative, we can conclude both points are saddle points. Since the determinant on $(\pm2/3,0)$ is positive we can conclude they are extrema. Since $H(f)_{xx}$ on $(2/3,0)$ is negative and positive on $(-2/3,0)$, they are a maximum and minimum respectively.

# 13

$f(x,y)=x^4+y^4-4xy$

$\nabla f=\langle4x^3-4y,4y^3-4x\rangle$

$\nabla f=\langle0,0\rangle\iff\begin{cases}4x^3-4y=0\\4y^3-4x=0\end{cases}$
$=\begin{cases}y=x^3\\x=y^3\end{cases}$
$=\begin{cases}y=y^9\\x=x^9\\x=y^3\end{cases}$
$\iff(x,y)\in\{(-1,-1),(0,0),(1,1)\}$

$H(f)=\begin{bmatrix}12x^2&-4\\-4&12y^2\end{bmatrix}$
$|H(f)|=144x^2y^2-16$

$\bigg|_{(-1,-1)}=128$
$\bigg|_{(0,0)}=-16$
$\bigg|_{(1,1)}=128$

Since the determinant on $\{(-1,-1),(1,1)\}$ is positive, they are extrema, and since $H(f)_{xx}$ for both are positive, they are both local minima. Since the determinant on $(0,0)$ is negative, it is a saddle point.

# 23

$f(x,y)=(x+3y)e^{y-x^2}$

$\nabla f=\langle(-2x(x+3y)+1)e^{y-x^2},(x+3y+3)e^{y-x^2}\rangle$

$\nabla f=\langle0,0\rangle\iff\begin{cases}(-2x(x+3y)+1)e^{y-x^2}=0\\(x+3y+3)e^{y-x^2}=0\end{cases}$
$=\cases e^{y-x^2}=0$ or $\begin{cases}-2x^2-6xy+1=0\\x+3y+3=0\end{cases}$
$=\cases y-x^2=-\infty$ or $\begin{cases}-2(-3y-3)^2-6(-3y-3)y+1=0\\x=-3y-3\end{cases}$
$=\begin{cases}-17-18y=0\\x=-3y-3\end{cases}$
$=\begin{cases}y=-17/18\\x=-1/6\end{cases}$
$\iff(x,y)=(-1/6,-17/18)$

$H(f)=\begin{bmatrix}(-2x(-2x(x+3y)+1)+(-4x-6y))e^{y-x^2}&(-2x(x+3y)+1-6x))e^{y-x^2}\\(-2x(x+3y+3)+1)e^{y-x^2}&(x+3y+6)e^{y-x^2}\end{bmatrix}$
$=\begin{bmatrix}(4x^3+12x^2y-6x-6y)e^{y-x^2}&(-2x^2-6xy-6x+1))e^{y-x^2}\\(-2x^2-6xy-6x+1)e^{y-x^2}&(x+3y+6)e^{y-x^2}\end{bmatrix}$

$|H(f)|=(4x^3+12x^2y-6x-6y)(x+3y+6)e^{2(y-x^2)}-(-2x^2-6xy-6x+1))^2e^{2(y-x^2)}$

$\bigg|_{(-1/6,-17/18)}\approx 2.57520028958$

Since the determinant at $(-1/6,-17/18)$ is positive and $H(f)_{xx}\approx 2.39552992222$ is also positive, it is a local minima.

# 29

$f(x,y)=x+y$

$0\le x\le 1$
$0\le y\le 1$

Since $f$ is always increasing on both $x$ and $y$, the bigger the value of $x$ and the bigger the value of $y$, the bigger the value of $f$. $1$ would maximize the value of both $x$ and $y$ as it is the maximum on the domain. $-1$ would minimize both $x$ and $y$ as it is the minimum.

Min: $(-1,-1)$
Max: $(1,1)$

# 37

$f(x,y)=xy$

$\nabla f=\langle y,x\rangle$

$\nabla f=\langle0,0\rangle\iff (x,y)=(0,0)$

$H(f)=\begin{bmatrix}0&1\\1&0\end{bmatrix}$
$|H(f)|=-1$

# 39

# 41
