---
date created: 2023-10-30 14:44
---

# 5

$f(x,y)=x^2+y^2$
$g(x,y)=2x+3y-6=0$

$\nabla f=\langle 2x,2y\rangle=\lambda\nabla g=\lambda\langle2,3\rangle$

$=\begin{cases}2x=2\lambda\\2y=3\lambda\\2x+3y=6\end{cases}$
$=\begin{cases}x=\lambda\\y=3\lambda/2\\13\lambda=12\end{cases}$
$=\begin{cases}x=12/13\\y=18/13\\\lambda=12/13\end{cases}$

$(x,y)=(12/13,18/13)$

$\text{Tangent}=\langle2,3\rangle\times\langle0,0,1\rangle=\langle3,-2\rangle$
$\text{Derivative along g}=\langle3,-2\rangle\cdot\langle2x,2y\rangle=6x-4y$
$\text{2nd der. along g}=\langle3,-2\rangle\nabla (6x-4y)=\langle3,-2\rangle\cdot\langle6,-4\rangle=26$

Since the 2nd derivative is positive, there is a minimum at $(12/13,18/13,36/13)$

# 7

$f(x,y)=xy$
$g(x,y)=4x^2+9y^2-32=0$

$\nabla f=\langle y,x\rangle=\lambda\nabla g=\lambda\langle8x,18y\rangle$

$=\begin{cases}y=8\lambda x\\x=18\lambda y\\4x^2+9y^2=32\end{cases}$
$=\begin{cases}y=8\lambda x\\x=18\lambda y\\x=144\lambda^2 x\\\lambda=\pm1/12\\4x^2+9y^2=32\end{cases}$
$=\begin{cases}y=\pm2x/3\\x=\pm3y/2\\8x^2=32\end{cases}$
$=\begin{cases}y=\pm2x/3\\x=\pm3y/2\\x=\pm2\\y=\pm4/3\end{cases}$

$\text{Tangent of g}=\langle18y,-8x\rangle$

| Point           | Tangent                 | 1st D.D.   | Nabla of D.D.           | 2nd D.D. | Max/Min |
| --------------- | ----------------------- | ---------- | ----------------------- | -------- | ------- |
| $(-2,-4/3,8/3)$ | $\langle-24,16\rangle$  | $16x-24y$  | $\langle16,-24\rangle$  | -768     | Max     |
| $(-2,4/3,-8/3)$ | $\langle24,16\rangle$   | $16x+24y$  | $\langle16,24\rangle$   | 768      | Min     |
| $(2,-4/3,-8/3)$ | $\langle-24,-16\rangle$ | $-16x-24y$ | $\langle-16,-24\rangle$ | 768      | Min     |
| $(2,4/3,8/3)$   | $\langle24,-16\rangle$  | $24y-16x$  | $\langle-16,24\rangle$  | -768     | Max     |

There are maxima at $(-2,-4/3,8/3)$ and $(2,4/3,8/3)$ and minima at $(-2,4/3,-8/3)$ and $(2,-4/3,-8/3)$

# 9

$f(x,y)=x^2+y^2$
$g(x,y)=x^4+y^4-1=0$

$\nabla f=\langle2x,2y\rangle=\lambda\nabla g=\lambda\langle4x^3,4y^3\rangle$

$=\begin{cases}2x=\lambda 4x^3\\2y=\lambda 4y^3\\x^4+y^4=1\end{cases}$
$=\begin{cases}1=\lambda 2x^2\\1=\lambda 2y^2\\x^4+y^4=1\end{cases}$
or $(x,y)\in\{(0,\pm1)\cup(\pm1,0)\}$
$=\begin{cases}y=x=\pm\sqrt{1/2\lambda}\\1/\lambda^2=2\end{cases}$
$=\begin{cases}y=x=\pm1/\sqrt[4]2\\\lambda=\pm\sqrt{1/2}\end{cases}$

$f(\pm1/\sqrt[4]2,\pm1/\sqrt[4]2)=\sqrt2$
$f(\{(0,\pm1)\cup(\pm1,0)\})=1$

Maximum: $\sqrt2$
Minimum: $1$

# 13

$f(x,y,z)=xy+2z$
$g(x)=x^2+y^2+z^2-36=0$

$\nabla f=\langle y,x,2\rangle=\lambda\nabla g=\lambda\langle2x,2y,2z\rangle$

$=\begin{cases}y=2\lambda x\\x=2\lambda y\\2=2\lambda z\\x^2+y^2+z^2=36\end{cases}$
$=\begin{cases}y=x\\\lambda=\pm1/2\\z=\pm2\\x^2=32/2\end{cases}$
$=\begin{cases}\lambda=\pm1/2\\z=\pm2\\y=x=\pm4\end{cases}$

$\iff(x,y,z)=(\pm4,\pm4,\pm2)|x=y$

$f(4,4,2)=20$
$f(-4,-4,2)=20$
$f(4,4,-2)=-20$
$f(-4,-4,-2)=-20$

Maximums at $(4,4,2)=20$ and $(-4,-4,2)=20$.
Minimums at $(4,4,-2)=-20$ and $(-4,-4,-2)=-20$

# 21

$f(x,y)=x$
$g(x,y)=x^2+6y^2+3xy-40=0$

$\nabla f=\langle1,0\rangle=\lambda\nabla g=\lambda\langle2x+3y,12y+3x\rangle$

$\begin{cases}x^2+6y^2+3xy=40\\\lambda2x+\lambda3y=1\\\lambda12y+\lambda3x=0\end{cases}$
$\begin{cases}x^2+6y^2+3xy=40\\x=-3y/2+1/2\lambda\\x=-4y\end{cases}$
$\begin{cases}y=\pm2\\x=-3y/2+1/2\lambda\\x=\mp8\end{cases}$

$(x,y)=(8,-2)$ has the greatest $x$ value

# 33

$\begin{cases}V=54\pi\\V=\pi r^2h\\S=2\pi rh+2\pi r^2\end{cases}$

$f(r,h)=2\pi rh+2\pi r^2$
$g(r,h)=\pi r^2h-54\pi=0$

$\nabla f=\langle2\pi h+4\pi r,2\pi r\rangle=\lambda\nabla g=\lambda\langle2\pi rh,\pi r^2\rangle$

$=\begin{cases}2\pi h+4\pi r=\lambda2\pi rh\\2\pi r=\lambda\pi r^2\\\pi r^2h=54\pi\end{cases}$
$=\begin{cases}h+2r=\lambda rh\\2=\lambda r\\\pi r^2h=54\pi\end{cases}$
$=\begin{cases}h=2r\\2=\lambda r\\r^3=27\end{cases}$
$=\begin{cases}h=6\\\lambda=2/3\\r=3\end{cases}$

$(r,h)=(3,6)$

# 41

$f(x,y,z)=x^2+y^2+z^2$
$g(x,y,z)=x+y+z-1=0$
$h(x,y,z)=x+2y+3z-6=0$

$\nabla f=\langle2x,2y,2z\rangle$
$\nabla g=\langle1,1,1\rangle$
$\nabla h=\langle1,2,3\rangle$

$\nabla f=\lambda\nabla g+\mu\nabla h$

$=\begin{cases}2x=\lambda+\mu\\2y=\lambda+2\mu\\2z=\lambda+3\mu\\x+y+z=1\\x+2y+3z=6\end{cases}$
$=\begin{cases}2x=\lambda+\mu\\2y=\lambda+2\mu\\2z=\lambda+3\mu\\3\lambda+6\mu=2\\3\lambda+7\mu=6\end{cases}$
$=\begin{cases}x=-5/3\\y=1/3\\2z=\lambda+3\mu\\\lambda=-22/3\\\mu=4\end{cases}$

# 53

# 55

# 56
