# 1

$\oint\limits_C\langle xy,y\rangle d\vec r$
$=\int\limits_0^{2\pi}\langle \cos t\sin t,\sin t\rangle\cdot\langle -\sin t,\cos t\rangle dt$
$=\int\limits_0^{2\pi}-\cos t\sin^2 t+\sin t\cos t ~ dt$
$=\bigg|_0^{2\pi}-\frac{\sin^3 t}{3}+\frac{\sin^2 t}{2}~ dt$
$=0$

$=\iint\limits_D 0-x~dA$
SInce $A$ is symmetric over $x$ and $F$ is even, the integral is $0$
$=0$

# 3

$\oint\limits_C\langle y^2,x^2\rangle$
$\iint\limits_D2x-2y~dA$
$\bigg|\bigg|_Dyx^2-xy^2~dA$
$=1-1$
$=0$

# 5

$\oint\limits_C\langle5y,2x\rangle$
$=\iint\limits_D2-5~dA$
$=\iint\limits_D-3~dA$
$=2*1*0.5*-3$
$=-3$

# 7

$\oint\limits_C\langle x^2y,0\rangle$
$=\iint\limits_D-x^2~dA$
$=\int\limits_0^{2\pi}\int\limits_0^1-r^3\cos^2\theta~drd\theta$
$=\int\limits_0^{2\pi}-\frac{1}{4}\cos^2\theta~d\theta$
$=\int\limits_0^{2\pi}-\frac{1}{4}(\frac{1}{2}+\frac{\cos(2\theta)}{2})~d\theta$
$=\bigg|_0^{2\pi}-\frac{1}{4}(\frac{1}{2}\theta+\frac{\sin(2\theta)}{2})~d\theta$
$=\frac{\pi}{4}$

# 11

$\oint\limits_C\langle x^{x+y},e^{x-y}\rangle$
$=-\iint\limits_De^{x-y}-e^{x+y}~dA$
$=-\int\limits_0^2\int\limits_y^{y+2} e^{x-y}-e^{x+y}~dxdy$
$=\int\limits_0^2 e^{2y+2}-e^{2y}+1-e^{2}~dy$
$=\frac{1}{2}e^{6}-\frac{1}{2}e^2-\frac{1}{2}e^{4}+\frac{1}{2}+2-2e^{2}$
$=\frac{1}{2}e^{6}-\frac{5}{2}e^2-\frac{1}{2}e^{4}+\frac{5}{2}$
$=\frac{1}{2}(e^4-5)(e^2-1)$

# 13

## a

$\nabla f=\langle 2xe^y,x^2e^y\rangle$
$f=x^2e^y$

## b

$\vec r=\langle t,0\rangle$
$\oint\limits_{OA}\langle0,t\rangle\cdot\langle 1,0\rangle dt$
$=0$

$\vec r=\langle0,t\rangle$
$\oint\limits_{OB}\langle0,0\rangle\cdot\langle 0,1\rangle dt$
$=0$

## c

$\oint\limits_C\vec F\cdot d\vec r$
$=\oint\limits_C(\nabla f+\vec G)\cdot d\vec r$
$=f(B)-f(A)+\oint\limits_C\vec G\cdot d\vec r$
$=f(B)-f(A)+\iint\limits_D1~dA-\oint\limits_{BO}\langle0,0\rangle\cdot\langle 0,1\rangle dt-\oint\limits_{OA}\langle0,t\rangle\cdot\langle 1,0\rangle dt$
$=f(B)-f(A)+\frac{16\pi}{4}$
$=f(B)-f(A)+4\pi$

$=4\pi-16$
