# 4.43

## a

$\text{Cov}(X_1+X_2,X_2+X_3)=E((X_1+X_2)(X_2+X_3))-E(X_1+X_2)E(X_2+X_3)$
$=E(X_1X_2)+E(X_1X_3)+E(X_2X_2)+E(X_2X_3)-(2\mu)(2\mu)$
$=+E(X_1)E(X_2)+E(X_1)E(X_3)+\text{Cov}(X_2,X_2)+E(X_2)E(X_3)+E(X_2)E(X_3)-4\mu^2$
$=\mu^2+\mu^2+\sigma^2+\mu^2+\mu^2-4\mu^2$
$=\sigma^2$

## b

$\text{Cov}(X_1+X_2,X_1-X_2)=E((X_1+X_2)(X_1-X_2))-E(X_1+X_2)E(X_1-X_2)$
$=E(X_1X_1-X_1X_2+X_2X_1-X_2X_2)$
$=E(X_1X_1)-E(X_2X_2)$
$=E(X_1X_1)-E(X_2X_2)$
$=\sigma^2-\sigma^2$
$=0$

# 4.45

## a

$f(x,y)=\frac{1}{2\pi\sigma_X\sigma_Y\sqrt{1-\rho^2}}\exp\left( -\frac{1}{2(1-\rho^2)}\left( \left( \frac{x-\mu_X}{\sigma_X} \right)^2 -2\rho \left( \frac{x-\mu_x}{\sigma_X} \right)\left( \frac{y-\mu_Y}{\sigma_Y} \right) + \left( \frac{y-\mu_Y}{\sigma_Y} \right)^2 \right) \right)$

$z_X=\frac{x-\mu_X}{\sigma_X}$
$z_Y=\frac{y-\mu_Y}{\sigma_Y}$

$f(x,y)=\frac{1}{2\pi\sigma_X\sigma_Y\sqrt{1-\rho^2}}\exp\left( -\frac{z_X^2 -2\rho z_Xz_Y + z_Y^2}{2(1-\rho^2)}\right)$
$f(x,y)=\frac{1}{2\pi\sigma_X\sigma_Y\sqrt{1-\rho^2}}\exp\left( -\frac{(z_X -\rho z_Y)^2 + z_Y^2(1- \rho^2) }{2(1-\rho^2)}\right)$
$f(x,y)=\frac{1}{\sqrt{2\pi}\sigma_Y\sqrt{1-\rho^2}}\exp\left( -\frac{z_Y^2}{2} \right) \frac{1}{\sqrt{2\pi}\sigma_X}\exp\left( -\frac{(z_X -\rho z_Y)^2}{2(1-\rho^2)}\right)$

$f_Y(u)=\int_{-\infty}^\infty f(x,y)~dx$
$f_Y(u)=\frac{1}{\sqrt{2\pi}\sigma_Y\sqrt{1-\rho^2}}\exp\left( -\frac{z_Y^2}{2} \right) \int_{-\infty}^\infty \frac{1}{\sqrt{2\pi}\sigma_X}\exp\left( -\frac{(z_X -\rho z_Y)^2}{2(1-\rho^2)}\right)~dx$

$dx_X\sigma_X=dx$
$f_Y(u)=\frac{1}{\sqrt{2\pi}\sigma_Y}\exp\left( -\frac{z_Y^2}{2} \right) \int_{-\infty}^\infty \frac{1}{\sqrt{2\pi}\sqrt{1-\rho^2}}\exp\left( -\frac{(z_X -\rho z_Y)^2}{2\sqrt{1-\rho^2}^2}\right)~dz$
$f_Y(u)=\frac{1}{\sqrt{2\pi}\sigma_Y}\exp\left( -\frac{z_Y^2}{2} \right)$

$Y\sim\text{N}(\mu_Y,\sigma^2_Y)$

The exact same is true for $X$, just replacing $_X$ variables with $_Y$

## b

## c

# 5.3

# 5.5

# 5.6
