# 2.1

## a

$Y=X^3$ and $f_X(x)=42x^5(1-x),\quad0<x<1$

$Y$ is increasing on the interval $(0,1)$, so we will not need to split the pdf into a piecewise

$f_Y(y)=f_X(g^{-1}(y))|\frac{d}{dy}g^{-1}(y)|$

$g(x)=x^3$
$Y=g(X)=X^3$
$g^{-1}(y)=\sqrt[3]{y}$
$\frac{d}{dy}g^{-1}(y)=y^{-2/3}/3$

$f_Y(y)=f_X(\sqrt[3]{y})|y^{-2/3}/3|$
$f_Y(y)=42(\sqrt[3]{y})^5(1-(\sqrt[3]{y}))|y^{-2/3}/3|$
$f_Y(y)=42y^{5/3}(1-\sqrt[3]{y})|y^{-2/3}/3|$
$f_Y(y)=(42y^{5/3}-42y^2)|y^{-2/3}/3|$

$y^{-2/3}$ is always positive

$f_Y(y)=(42y^{5/3}-42y^2)(y^{-2/3}/3)$
$f_Y(y)=14(y-y^{4/3})$
$f_Y(y)=14y(1-y^{1/3})$
$\square$

$\int\limits_0^1f_Y(y)dy=\int\limits_0^1 14y(1-y^{1/3})dy$
$=14\int\limits_0^1y-y^{4/3}$
$=14(y^2/2-3y^{7/3}/7)\bigg\vert_0^1$
$=7y^2-6y^{7/3}\bigg\vert_0^1$
$=7-6-0+0=1$
$\square$
## b

$Y=4X+3$ and $f_X(x)=7e^{-7x},\quad0<x<\infty$

$Y$ is increasing on the interval $(0,\infty)$, so we will not need to split the pdf into a piecewise

$f_Y(y)=f_X(g^{-1}(y))|\frac{d}{dy}g^{-1}(y)|$

$g(x)=4x+3$
$g^{-1}(y)=y/4-3/4$
$\frac{d}{dy}g^{-1}(y)=1/4$

$f_Y(y)=f_X(y/4-3/4)|1/4|$
$f_Y(y)=7e^{-7(y/4-3/4)}/4$
$f_Y(y)=7e^{21/4-7y/4}/4,\quad3<y<\infty$
$\square$

$\int\limits_3^\infty7e^{21/4-7y/4}/4dy$
$-e^{21/4-7y/4}\bigg\vert_3^\infty$
$=0+e^0=1$
$\square$

## c

$Y=X^2$ and $f_X(X)=30x^2(1-x)^2,\quad 0<x<1$

$Y$ is increasing on the interval $(0,1)$, so we will not need to split the pdf into a piecewise

$f_Y(y)=f_X(g^{-1}(y))|\frac{d}{dy}g^{-1}(y)|$

$g(x)=x^2$
$Y=g(X)=X^2$
$g^{-1}(y)=\sqrt{y}$
$\frac{d}{dy}g^{-1}(y)=y^{-1/2}/2$

$f_Y(y)=f_X(\sqrt{y})|y^{-1/2}/2|$
$f_Y(y)=30\sqrt{y}^2(1-\sqrt{y})^2|y^{-1/2}/2|$
$f_Y(y)=15\sqrt y(1-\sqrt{y})^2$
$f_Y(y)=15\sqrt y(1-2\sqrt{y}+y)$
$f_Y(y)=15(\sqrt y-2y+y^{3/2})$
$\square$

$\int\limits_0^1 15(\sqrt y-2y+y^{3/2})dy$
$15(2y^{3/2}/3-y^2+2y^{5/2}/5)\bigg\vert_0^1$
$=15(2/3-1+2/5)$
$=15(10/15-15/15+6/16)$
$=1$
$\square$

# 2.3

$f_X(x)=(2/3)^x/3,\quad x=0,1,2,...$
$f_Y(y)=f_X(g^{-1}(y))|\frac{d}{dy}g^{-1}(y)|$

$g(x)=x/(x+1)$
$yx+y-x=0$
$x(y-1)=-y$
$g^{-1}(y)=y/(1-y)$
$\frac{d}{dy}g^{-1}(y)=((1)(1-y)-(-1)(y))/(1-y)^2$
$\frac{d}{dy}g^{-1}(y)=1/(1-y)^2$

$f_Y(y)=f_X(y/(1-y))|1/(1-y)^2|,\quad y=0,1/2,2/3,3/4,4/5,...$
$f_Y(y)=(2/3)^{y/(1-y)}/3(1-y)^2,\quad y=0,1/2,2/3,3/4,4/5,...$

# 2.6

## a

$f_X(x)=e^{-|x|}/2,\quad -\infty<x<\infty;Y=|X|^3$
$f_Y(y)=f_X(g^{-1}(y))|\frac{d}{dy}g^{-1}(y)|$

$g(x)=|x|^3$
$g^{-1}(y)=\pm\sqrt[3]y,\quad 0\le y$
$\frac{d}{dy}g^{-1}(y)=\pm y^{-2/3}/3$

$f_Y(y)=f_X(\pm\sqrt[3]y)(y^{-2/3}/3)$
$f_Y(y)=y^{-2/3}e^{-|\pm\sqrt[3]y|}/6$
$\square$

$\int\limits_0^\infty y^{-2/3}e^{-|\pm\sqrt[3]y|}/6dy$
$2\int\limits_0^\infty y^{-2/3}e^{-\sqrt[3]y}/6dy$
$2(-e^{-\sqrt[3]y}/2)\bigg\vert_0^\infty$
$-e^{-\sqrt[3]y}\bigg\vert_0^\infty$
$=0--1$
$1$
$\square$

## b

$f_X(x)=3(x+1)^2/8,\quad-1<x<1;Y=1-X^2$
$f_Y(y)=f_X(g^{-1}(y))|\frac{d}{dy}g^{-1}(y)|$

$g(x)=1-x^2$
$g^{-1}(y)=\pm\sqrt{1-y},\quad0<y<1$
$\frac{d}{dy}g^{-1}(y)=\mp(1-y)^{-1/2}/2$

$f_Y(y)=f_X(\pm\sqrt{1-y})|\mp(1-y)^{-1/2}/2|$
$f_Y(y)=3((\pm\sqrt{1-y})+1)^2((1-y)^{-1/2}/2)/8$
$\square$

$\int\limits_0^1f_Y(y)dy=\begin{cases}\int\limits_0^1((-\sqrt{1-y})+1)^3/8dy&\text{for x>0}\\\int\limits_1^0((+\sqrt{1-y})+1)^3/8dy&\text{for x<0}\end{cases}$
$=1/8-0+1-1/8$
$=1$
$\square$

## c

$f_X(x)=3(x+1)^2/8,\quad-1<x<1;Y=1-X^2\text{ if }X\le0; Y=1-X\text{ if }X>0$
$f_Y(y)=f_X(g^{-1}(y))|\frac{d}{dy}g^{-1}(y)|$

$g(x)=\begin{cases}1-x^2&x\le0\\1-x&x>0\end{cases}$
$g^{-1}(x)=\begin{cases}-\sqrt{1-y}&x\le0;0\le y<1\\1-y&x>0;1>y>0\end{cases}$
$\frac{d}{dy}g^{-1}(x)=\begin{cases}(1-y)^{-1/2}/2&x\le0;0\le y<1\\-1&x>0;1>y>0\end{cases}$

$f_Y(y)=f_X(g^{-1}(y))|\frac{d}{dy}g^{-1}(y)|$
$g^{-1}(x)=\begin{cases}f_X(-\sqrt{1-y})|(1-y)^{-1/2}/2|&x\le0;0\le y<1\\f_X(1-y)|-1|&x>0;1>y>0\end{cases}$
$g^{-1}(x)=\begin{cases}  3(-\sqrt{1-y}+1)^2|(1-y)^{-1/2}/2|/8&x\le0;0\le y<1\\3(1-y+1)^2/8&x>0;1>y>0\end{cases}$
$g^{-1}(x)=\begin{cases}3(-\sqrt{1-y}+1)^2(1-y)^{-1/2}/16&x\le0;0\le y<1\\3(2-y)^2/8&x>0;1>y>0\end{cases}$
$\square$

$\int f_Y(y)dy=\begin{cases}\int3(-\sqrt{1-y}+1)^2(1-y)^{-1/2}/16dy&x\le0;0\le y<1\\\int3(2-y)^2/8dy&x>0;1>y>0\end{cases}$
$\int f_Y(y)dy=\begin{cases}(-\sqrt{1-y}+1)^3/8&x\le0;0\le y<1\\(2-y)^3/8&x>0;1>y>0\end{cases}$
$\int\limits_0^1 f_Y(y)dy=\begin{cases}(-\sqrt{1-y}+1)^3/8\bigg\vert_0^1&x\le0;0\le y<1\\(2-y)^3/8\bigg\vert_1^0&x>0;1>y>0\end{cases}$
$=1/8-0+1-1/8$
$=1$
$\square$

# 2.9

$f_X(x)=\begin{cases}(x-1)/2&1<x<3\\0&\text{otherwise}\end{cases}$
$f_Y(y)=\begin{cases}1&0\le y\le1\\0&\text{otherwise}\end{cases}$

$F_X(x)=\begin{cases}0&x\le1\\(x-1)^2/4&1<x<3\\1&3\le x\end{cases}$
$F_Y(y)=\begin{cases}0&x\le0\\x&0<y<1\\1&1\le x\end{cases}$

$F_Y(y)=F_X(g^{-1}(y$
