---
date created: 2023-10-05 21:44
date updated: 2023-10-05 21:45
---

# 2.17

## a

$f(x)=3x^2\qquad,0<x<1$

$P(X>m)=P(X<m)$
$F(m)=1-F(m)$
$F(m)=0.5$

$F(x)=\int\limits_0^xf(t)dt$
$F(x)=x^3$
$0.5=m^3$
$m=0.7937$

## b

$f(x)=\frac{1}{\pi(1+x^2)}\qquad,-\infty<x<\infty$

$P(X>m)=P(X<m)$
$F(m)=1-F(m)$
$F(m)=0.5$

$F(x)=\int\limits_{-\infty}^xf(t)dt$
$F(x)=\arctan (x)/\pi+0.5$
$0.5=\arctan(m)/\pi+0.5$
$m=0$

# 2.24

## a

$f(x)=ax^{a-1}\qquad,0<x<1,a>0$

### $EX$

$EX=\int\limits_0^1 xf(x)dx$
$EX=\int\limits_0^1ax^adx$
$EX=\frac{ax^{a+1}}{a+1}\bigg\vert_0^1$
$EX=\frac{a}{a+1}$

### $EX^2$

$EX^2=\int\limits_0^1x^2f(x)dx$
$EX^2=\int\limits_0^1ax^{a+1}dx$
$EX^2=\frac{ax^{a+2}}{a+2}\bigg\vert_0^1$
$EX^2=\frac{a}{a+2}$

### $\sigma^2$

$\sigma^2=EX^2-(EX)^2$
$\sigma^2=\frac{a}{a+2}-(\frac{a}{a+1})^2$
$\sigma^2=\frac{a}{a+2}-\frac{a^2}{(a+1)^2}$
$\sigma^2=\frac{a^3+2a^2+a}{(a+2)(a+1)^2}\frac{a^3+2a^2}{(a+2)(a+1)^2}$
$\sigma^2=\frac{a}{(a+2)(a+1)^2}$

## b

$f(x)=1/n\qquad,x=1,2,...,n,n>0 \text{ an integer}$

### $EX$

$EX=\sum\limits_{x=1}^n xf(x)$
$EX=\sum\limits_{x=1}^n x/n$
$EX=n(n+1)/2n$
$EX=(n+1)/2$

### $EX^2$

$EX^2=\sum\limits_{x=1}^nx^2f(x)$
$EX^2=\sum\limits_{x=1}^n x^2/n$
$EX^2=(n+1)(2n+1)/6$

### $\sigma^2$

$\sigma^2=EX^2-(EX)^2$
$\sigma^2=(n+1)(2n+1)/6-((n+1)/2)^2$
$\sigma^2=\frac{2(n+1)(2n+1)-3(n+1)^2}{12}$
$\sigma^2=\frac{n^2-1}{12}$

## c

$f(x)=3(x-1)^2/2\qquad ,0<x<2$

### $EX$

$EX=\int\limits_0^2 xf(x)dx$
$EX=\frac{3}{2}\int\limits_0^2x^3-2x^2+xdx$
$EX=\frac{3}{2}(x^4/4-2x^3/3+x^2/2)\bigg\vert_0^2$
$EX=1$

### $EX^2$

$EX^2=\int\limits_0^2 x^2f(x)dx$
$EX^2=\frac{3}{2}\int\limits_0^2x^4-2x^3+x^2dx$
$EX^2=\frac{3}{2}(x^5/5-x^4/2+x^3/3)\bigg\vert_0^2$
$EX^2=8/5$

### $\sigma^2$

$\sigma^2=EX^2-(EX)^2$
$\sigma^2=8/5-1$
$\sigma^2=3/5$

# 2.28

## b

$f(x)=e^{-x}\qquad,x\ge0$

### $EX$

$EX=\int\limits_0^\infty xe^{-x}dx$

| u   | dv        |
| --- | --------- |
| $x$ | $e^{-x}$  |
| $1$ | $-e^{-x}$ |
| $0$ | $e^{-x}$  |

$EX=-xe^{-x}-e^{-x}\bigg\vert_0^\infty$
$EX=1$

### $\mu_2$

$\mu_2=E((X-\mu)^2)$
$\mu_2=\int\limits_0^\infty(x-1)^2e^{-x}dx$
$\mu_2=\int\limits_0^\infty(x^2-2x+1)e^{-x}$
$\mu_2=-(x^2+2x+2-2x-2+1)e^{-x}\bigg\vert_0^\infty$
$\mu_2=-(x^2+1)e^{-x}\bigg\vert_0^\infty$
$\mu_2=1$

### $\mu_3$

$\mu_3=E((X-\mu)^3)$
$\mu_3=\int\limits_0^\infty(x-1)^3e^{-x}dx$
$\mu_3=\int\limits_0^\infty(x^3-3x^2+3x-1)e^{-x}$
$\mu_3=-(x^3+3x^2+6x+6-3x^2-6x-6+3x+3-1)e^{-x}\bigg\vert_0^\infty$
$\mu_3=-(x^3+3x+2)e^{-x}\bigg\vert_0^\infty$
$\mu_3=2$

### $\alpha_3$

$\alpha_3=\frac{\mu_3}{\mu_2^{3/2}}$
$\alpha_3=2$

## c

### i

$f(x)=\frac{1}{\sqrt{2\pi}}e^{-x^2/2}$

#### $\mu$

$EX=\int\limits_{-\infty}^\infty xf(x)dx$
$EX=\int\limits_{-\infty}^\infty x\frac{1}{\sqrt{2\pi}}e^{-x^2/2}dx$
$EX=0$

#### $\mu_2$

$\mu_2=E((X-\mu)^2)$
$\mu_2=\int\limits_{-\infty}^\infty x^2\frac{1}{\sqrt{2\pi}}e^{-x^2/2}dx$
$\mu_2=1$

#### $\mu_4$

$\mu_4=E((X-\mu)^4)$
$\mu_4=\int\limits_{-\infty}^\infty x^4\frac{1}{\sqrt{2\pi}}e^{-x^2/2}dx$
$\mu_4=3$

#### $\alpha_4$

$\alpha_4=\frac{\mu^4}{\mu_2^2}$
$\alpha_4=3$

The graph does not look very peaked to me

### ii

$f(x)=1/2$

#### $\mu$

$EX=\int\limits_{-1}^1 xf(x)dx$
$EX=\int\limits_{-1}^1 x/2dx$
$EX=0$

#### $\mu_2$

$\mu_2=E((X-\mu)^2)$
$\mu_2=\int\limits_{-1}^1 x^2/2dx$
$\mu_2=1/3$

#### $\mu_4$

$\mu_4=E((X-\mu)^4)$
$\mu_4=\int\limits_{-1}^1 x^4/2dx$
$\mu_4=1/5$

#### $\alpha_4$

$\alpha_4=\frac{\mu^4}{\mu_2^2}$
$\alpha_4=9/5$

This graph does not look peaked at all

### iii

$f(x)=1/2e^{-|x|}$

#### $\mu$

$EX=\int\limits_{-\infty}^\infty xf(x)dx$
$EX=\int\limits_{-\infty}^\infty x/2e^{-|x|}dx$
$EX=0$

#### $\mu_2$

$\mu_2=E((X-\mu)^2)$
$\mu_2=\int\limits_{-\infty}^\infty x^2/2e^{-|x|}dx$
$\mu_2=2$

#### $\mu_4$

$\mu_4=E((X-\mu)^4)$
$\mu_4=\int\limits_{-\infty}^\infty x^4/2e^{-|x|}dx$
$\mu_4=24$

#### $\alpha_4$

$\alpha_4=\frac{\mu^4}{\mu_2^2}$
$\alpha_4=6$

This graph looks the most peaked compared to everything else

# 2.33

## c

### i

$M(x)=E(e^{tX})$
$M(x)=\sum\limits_{x=0}^\infty e^{tx}e^{-\lambda}\lambda^x/x!$
$M(x)=e^{-\lambda}\sum\limits_{x=0}^\infty e^{tx}\lambda^x/x!$
$M(x)=e^{-\lambda}e^{\lambda e^t}$
$M(x)=e^{\lambda e^t-\lambda}$
$M(x)=e^{\lambda(e^t-1)}$

#### $EX$

$EX=\frac{d}{dt}M(t)\bigg\vert_0$

$EX=e^{\lambda(e^t-1)}\lambda e^t\bigg\vert_0$
$EX=\lambda$

#### $EX^2$

$EX^2=\frac{d^2}{d^2t}M(t)\bigg\vert_0$

$EX^2=\frac{d}{dx}e^{\lambda(e^t-1)}\lambda e^t\bigg\vert_0$
$EX^2=\frac{d}{dx}e^{\lambda(e^t-1)}\lambda^2 e^2t+ e^{\lambda(e^t-1)}\lambda e^t\bigg\vert_0$
$EX^2=\lambda^2+\lambda$

#### $\sigma^2$

$\sigma^2=EX^2-(EX)^2$
$\sigma^2=\lambda^2+\lambda-(\lambda)^2$
$\sigma^2=\lambda$

### ii

$M(x)=E(e^{tX})$
$M(x)=\sum\limits_{x=0}^\infty e^{tx}p(1-p)^x$
$M(x)=p\sum\limits_{x=0}^\infty (e^t(1-p))^x$
$M(x)=p/(1-e^t(1-p))$

#### $EX$

$EX=\frac{d}{dt}M(t)\bigg\vert_0$
$EX=\frac{p(e^t(1-p))}{(1-e^t(1-p))^2}\bigg\vert_0$
$EX=\frac{1-p}{p}$

#### $EX^2$

$EX^2=\frac{d^2}{d^2t}M(t)\bigg\vert_0$
$EX^2=\frac{d}{dx}\frac{p(e^t(1-p))}{(1-e^t(1-p))^2}\bigg\vert_0$
$EX^2=\frac{d}{dx}\frac{pe^t-p^2e^t}{(1-e^t(1-p))^2}\bigg\vert_0$
$EX^2=\frac{(pe^t-p^2e^t)(1-e^t(1-p))^2+2(pe^t-p^2e^t)(1-e^t(1-p))(e^t(1-p))}{(1-e^t(1-p))^4}\bigg\vert_0$
$EX^2=\frac{(p-p^2)(p)^2+2(p-p^2)(p)(1-p)}{p^4}$
$EX^2=\frac{(p-p^2)+2(1-p)(1-p)}{p^2}$
$EX^2=\frac{p-p^2+2-4p+2p^2}{p^2}$
$EX^2=\frac{p^2-3p+2}{p^2}$
$EX^2=\frac{(p-2)(p-1)}{p^2}$

#### $\sigma^2$

$\sigma^2=EX^2-(EX)^2$
$\sigma^2=\frac{(p-2)(p-1)}{p^2}-(\frac{1-p}{p})^2$
$\sigma^2=\frac{(p-2)(p-1)-(1-p)^2}{p^2}$
$\sigma^2=\frac{1-p}{p^2}$

### iii

$M(x)=E(e^{tX})$
$M(x)=\int\limits_{-\infty}^\infty e^{tx}\frac{e^{-(x-\mu)^2/(2\sigma^2)}}{\sqrt{2\pi}\sigma}dx$
Let $u=x-\mu$ and $x=u+\mu$
$M(x)=\int\limits_{-\infty}^\infty e^{t(x+\mu)}\frac{e^{-u^2/(2\sigma^2)}}{\sqrt{2\pi}\sigma}du$
$M(x)=\frac{e^{t\mu}}{\sqrt{2\pi}\sigma}\int\limits_{-\infty}^\infty e^{tu}e^{-u^2/(2\sigma^2)}du$
$M(x)=\frac{e^{t\mu}}{\sqrt{2\pi}\sigma}\int\limits_{-\infty}^\infty e^{(2tu\sigma^2-u^2)/(2\sigma^2)}du$
$M(x)=\frac{e^{t\mu}}{\sqrt{2\pi}\sigma}\int\limits_{-\infty}^\infty e^{(-(u-t\sigma^2)^2+t^2\sigma^4)/(2\sigma^2)}du$
$M(x)=\frac{e^{t\mu}e^{\sigma^2t^2/2}}{\sqrt{2\pi}\sigma}\int\limits_{-\infty}^\infty e^{-(u-t\sigma^2)^2/(2\sigma^2)}du$
$M(x)=\frac{e^{t\mu}e^{\sigma^2t^2/2}}{\sqrt{2\pi}\sigma}\int\limits_{-\infty}^\infty e^{-(\frac{u-t\sigma^2}{\sqrt2\sigma})^2}du$
Let $v=\frac{u-t\sigma^2}{\sqrt2\sigma}$ and $dv=\frac{du}{\sqrt2\sigma}$ and $du=\sqrt2\sigma dv$
$M(x)=\frac{e^{t\mu}e^{\sigma^2t^2/2}}{\sqrt\pi}\int\limits_{-\infty}^\infty e^{-v^2}dv$
$M(x)=e^{t\mu}e^{\sigma^2t^2/2}$
$M(x)=e^{\mu t+\sigma^2t^2/2}z$

#### $EX$

$EX=\frac{d}{dt}M(t)\bigg\vert_0$
$EX=\frac{d}{dt}e^{\mu t+\sigma^2t^2/2}\bigg\vert_0$
$EX=(\mu+\sigma^2t)e^{\mu t+\sigma^2t^2/2}\bigg\vert_0$
$EX=\mu$

#### $EX^2$

$EX^2=\frac{d^2}{d^2t}M(t)\bigg\vert_0$
$EX=\frac{d}{dt}(\mu+\sigma^2t)e^{\mu t+\sigma^2t^2/2}\bigg\vert_0$
$EX=(\sigma^2+(\mu+\sigma^2t)^2)e^{\mu t+\sigma^2t^2/2}\bigg\vert_0$
$EX=\sigma^2+\mu^2$

#### $\sigma^2$

$\sigma^2=EX^2-(EX)^2$
$\sigma^2=\sigma^2+\mu^2-(\mu)^2$
$\sigma^2=\sigma^2$
