# 3.1

If $X\sim \text{DUniform}(N_0,N_1)$, then

## $EX$
$EX=\sum\limits_{n=N_0}^{N_1}n\frac{1}{N_1-N_0+1}$
$=\frac{1}{N_1-N_0+1}\sum\limits_{n=N_0}^{N_1}n$
$=\frac{1}{N_1-N_0+1}(\sum\limits_{n=0}^{N_1}n-\sum\limits_{n=0}^{N_0-1}n)$
$=\frac{1}{N_1-N_0+1}(\frac{N_1(N_1+1)}{2}-\frac{N_0(N_0-1)}{2})$
$=\frac{1}{N_1-N_0+1}\frac{N_1^2+N_1-N_0^2+N_0}{2}$
$=\frac{N_1^2+N_1-N_0^2+N_0}{2(N_1-N_0+1)}$
$=\frac{(N_0+N_1)(N_1-N_0+1)}{2(N_1-N_0+1)}$
$=\frac{N_0+N_1}{2}$
$\square$

## $EX^2$

$EX^2=\sum\limits_{n=N_0}^{N_1}n^2\frac{1}{N_1-N_0+1}$
$=\frac{1}{N_1-N_0+1}\sum\limits_{n=N_0}^{N_1}n^2$
$=\frac{1}{N_1-N_0+1}(\sum\limits_{n=0}^{N_1}n^2-\sum\limits_{n=0}^{N_0-1}n^2)$
$=\frac{1}{N_1-N_0+1}(\frac{N_1(N_1+1)(2N_1+1)}{6}-\frac{N_0(N_0-1)(2N_0-1)}{6})$
$=\frac{1}{N_1-N_0+1}\frac{2N_1^3+3N_1^2+N_1-2N_0^3+3N_0^2-N_0}{6}$
$=\frac{2N_1^3+3N_1^2+N_1-2N_0^3+3N_0^2-N_0}{6(N_1-N_0+1)}$
$=\frac{(N_1-N_0+1)(2N_0^2+2N_0N_1-N_0+2N_1^2+N_1)}{6(N_1-N_0+1)}$
$=\frac{2N_0^2+2N_0N_1-N_0+2N_1^2+N_1}{6}$

## $\text{Var}X$

$=\frac{2N_0^2+2N_0N_1-N_0+2N_1^2+N_1}{6}-(\frac{N_1+N_0}{2})^2$
$=\frac{2N_0^2+2N_0N_1-N_0+2N_1^2+N_1}{6}-\frac{N_1^2+2N_1N_0+N_0^2}{4}$
$=\frac{4N_0^2+4N_0N_1-2N_0+4N_1^2+2N_1-3N_1^2-6N_1N_0-3N_0^2}{12}$
$=\frac{N_0^2-2N_0N_1-2N_0+N_1^2+2N_1}{12}$
$=\frac{(N_1-N_0)(N_1-N_0+2)}{12}$
$\square$

# 3.5

$p=0.8$
$N=100$
$x=85$

This can be m

# 3.7

# 3.12

# 3.13
## a