# 3.22

## b

$X\sim\text{Binom}(r,p)$
$P(X=x)=\begin{pmatrix}n\\x\end{pmatrix}p^x(1-p)^{n-x}$

### $E(X)$

$E(X)=\sum\limits_{x\in X}xP(X=x)$
$E(X)=\sum\limits_{x=1}^nx\begin{pmatrix}n\\x\end{pmatrix}p^x(1-p)^{n-x}$
$E(X)=\sum\limits_{x=1}^nnp\frac{(n-1)!}{(x-1)!(n-x)!}p^{x-1}(1-p)^{n-x}$
$E(X)=np\sum\limits_{x=1}^n\begin{pmatrix}n-1\\x-1\end{pmatrix}p^{x-1}(1-p)^{n-x}$
Let $\tilde x=x-1\qquad\tilde n=n-1$
$E(X)=np\sum\limits_{\tilde x=0}^{\tilde n}\begin{pmatrix}\tilde n\\\tilde x\end{pmatrix}p^{\tilde x}(1-p)^{\tilde n-\tilde x}$
$E(X)=np$

### $E(X^2)$

$E(X^2)=\sum\limits_{x\in X}x^2P(X=x)$
$E(X^2)=\sum\limits_{x=1}^nx^2\begin{pmatrix}n\\x\end{pmatrix}p^x(1-p)^{n-x}$
$E(X^2)=np\sum\limits_{\tilde x=0}^{\tilde n}(\tilde x+1)\begin{pmatrix}\tilde n\\\tilde x\end{pmatrix}p^{\tilde x}(1-p)^{\tilde n-\tilde x}$
$E(X^2)=np(1+\sum\limits_{\tilde x=0}^{\tilde n}\tilde x\begin{pmatrix}\tilde n\\\tilde x\end{pmatrix}p^{\tilde x}(1-p)^{\tilde n-\tilde x})$
$E(X^2)=np(1+\tilde np)$
$E(X^2)=np(1+(n-1)p)$
$E(X^2)=np+n^2p^2-np^2$

### $\text{Var}(X)$

$\text{Var}(X)=E(X^2)-(E(X))^2$
$\text{Var}(X)=np+n^2p^2-np^2-(np)^2$
$\text{Var}(X)=np-np^2$
$\text{Var}(X)=np(1-p)$
$\square$

## c

$X\sim\text{Gamma}(\alpha,\beta)$
$f(x)=\frac{x^{\alpha-1}e^{-x/\beta}}{\Gamma(\alpha)\beta^\alpha}$

### $E(X)$

$E(X)=\int\limits_{-\infty}^\infty xf(x)dx$
$E(X)=\int\limits_0^\infty x\frac{x^{\alpha-1}e^{-x/\beta}}{\Gamma(\alpha)\beta^\alpha}dx$
$E(X)=\int\limits_0^\infty\alpha\beta\frac{x^{\alpha}e^{-x/\beta}}{\Gamma(\alpha+1)\beta^{\alpha+1}}dx$
$E(X)=\alpha\beta\int\limits_0^\infty f(x|\alpha+1,\beta)dx$
$E(X)=\alpha\beta$

### $E(X^2)$

$E(X^2)=\int\limits_{-\infty}^\infty x^2f(x)dx$
$E(X)=\int\limits_0^\infty x^2\frac{x^{\alpha-1}e^{-x/\beta}}{\Gamma(\alpha)\beta^\alpha}dx$
$E(X)=\alpha\beta\int\limits_0^\infty x\frac{x^{\alpha}e^{-x/\beta}}{\Gamma(\alpha+1)\beta^{\alpha+1}}dx$
$E(X)=\alpha\beta\int\limits_0^\infty (\alpha+1)\beta \frac{x^{\alpha+1}e^{-x/\beta}}{\Gamma(\alpha+2)\beta^{\alpha+2}}dx$
$E(X)=\alpha(\alpha+1)\beta^2\int\limits_0^\infty f(x|\alpha+2,\beta)dx$
$E(X)=\alpha(\alpha+1)\beta^2$
$E(X)=\alpha^2\beta^2+\alpha\beta^2$

### $\text{Var}(X)$

$\text{Var}(X)=E(X^2)-(E(X))^2$
$\text{Var}(X)=\alpha^2\beta^2+\alpha\beta^2-(\alpha\beta)^2$
$\text{Var}(X)=\alpha\beta^2$
$\square$

## e

$X\sim\text{DExp}(\mu,\sigma)$
$f(x)=\frac{e^{-|x-\mu|/\sigma}}{2\sigma}$

### $E(X)$

$E(X)=\int\limits_{-\infty}^\infty xf(x)dx$
$E(X)=\frac{1}{2\sigma}\int\limits_{-\infty}^\infty xe^{-|x-\mu|/\sigma}dx$
$E(X)=\frac{1}{2\sigma}(\int\limits_{-\infty}^\mu xe^{-|x-\mu|/\sigma}dx+\int\limits_{\mu}^\infty xe^{-|x-\mu|/\sigma}dx)$
$E(X)=\frac{1}{2\sigma}(\int\limits_{-\infty}^\mu xe^{(x-\mu)/\sigma}dx+\int\limits_{\mu}^\infty xe^{(\mu-x)/\sigma}dx)$
let $u=(x-\mu)/\sigma$ and $du=dx/\sigma$
let $v=(\mu-x)/\sigma$ and $dv=-dx/\sigma$
$E(X)=\frac{1}{2\sigma}(\int\limits_{-\infty}^0 \sigma (\sigma u+\mu)e^udu-\int\limits_{-\infty}^0\sigma(\sigma v-\mu)e^vdv)$
$E(X)=\frac{1}{2}(\sigma\int\limits_{-\infty}^0 ue^udu+\mu\int\limits_{-\infty}^0e^udu-\sigma\int\limits_{-\infty}^0ve^vdv+\mu\int\limits_{-\infty}^0e^vdv)$
$E(X)=\mu\int\limits_{-\infty}^0e^udu$
$E(X)=\mu\bigg(e^u\bigg|_{-\infty}^0\bigg)$
$E(X)=\mu(1)$
$E(X)=\mu$

### $E(X^2)$

$E(X^2)=\int\limits_{-\infty}^\infty x^2f(x)dx$
$E(X^2)=\frac{1}{2\sigma}\int\limits_{-\infty}^\infty x^2e^{-|x-\mu|/\sigma}dx$
$E(X^2)=\frac{1}{2\sigma}(\int\limits_{-\infty}^\mu x^2e^{-|x-\mu|/\sigma}dx+\int\limits_{\mu}^\infty x^2e^{-|x-\mu|/\sigma}dx)$
$E(X^2)=\frac{1}{2\sigma}(\int\limits_{-\infty}^\mu x^2e^{(x-\mu)/\sigma}dx+\int\limits_{\mu}^\infty x^2e^{(\mu-x)/\sigma}dx)$
let $u=(x-\mu)/\sigma$ and $du=dx/\sigma$
let $v=(\mu-x)/\sigma$ and $dv=-dx/\sigma$
$E(X^2)=\frac{1}{2\sigma}(\int\limits_{-\infty}^0 \sigma (\sigma u+\mu)^2e^udu+\int\limits_{-\infty}^0\sigma(\sigma v-\mu)^2e^vdv)$
$E(X^2)=\frac{1}{2}(\int\limits_{-\infty}^0(\sigma u+\mu)^2e^udu+\int\limits_{-\infty}^0(\sigma v-\mu)^2e^vdv)$
$E(X^2)=\int\limits_{-\infty}^0(\sigma^2 u^2+\mu^2)e^udu$
$E(X^2)=\sigma^2\int\limits_{-\infty}^0 u^2e^udu+\mu^2\int\limits_{-\infty}^0e^udu$
$E(X^2)=\sigma^2\int\limits_{-\infty}^0 u^2e^udu+\mu^2$

| $u$   | $dv$  |
| ----- | ----- |
| $u^2$ | $e^u$ |
| $2u$  | $e^u$ |
| $2$   | $e^u$ |
| $0$   | $e^u$ |

$E(X^2)=\sigma^2\bigg((u^2-2u+2)e^u\bigg|_{-\infty}^0\bigg)+\mu^2$
$E(X^2)=\sigma^2(2)+\mu^2$
$E(X^2)=2\sigma^2+\mu^2$

### $\text{Var}(X)$

$\text{Var}(X)=E(X^2)-(E(X))^2$
$\text{Var}(X)=2\sigma^2+\mu^2-(\mu)^2$
$\text{Var}(X)=2\sigma^2$
$\square$

# 3.24

## c

$X\sim\text{Gamma}(a,b)$
$Y=1/X$
$g(x)=1/x$
$g^{-1}(y)=1/y$

$F_Y(x)=F_X(y^{-1}(y))$
$f_Y(y)=f_X(g^{-1}(y)){g^{-1}}'(y)$

$f_X(x)=\frac{x^{\alpha-1}e^{-x/\beta}}{\Gamma(\alpha)\beta^\alpha}$
${g^{-1}}'(y)=-1/y^2$

$f_Y(y)=\frac{(1/y)^{\alpha-1}e^{-(1/y)/\beta}}{y^2\Gamma(\alpha)\beta^\alpha}$
$f_Y(y)=\frac{y^{-\alpha+1}e^{-(1/y)/\beta}}{y^2\Gamma(\alpha)\beta^\alpha}$
$f_Y(y)=\frac{y^{-\alpha-1}e^{-1/y\beta}}{\Gamma(\alpha)\beta^\alpha}$
$f_Y(y)=\frac{e^{-1/y\beta}}{\Gamma(\alpha)\beta^\alpha y^{\alpha+1}}\sim\text{IGamma}(\alpha,\beta)$

Which is the inverse Gamma distribution's PDF

If we use the substitution $\tilde\beta=1/\beta$ we get the more common form of the inverse Gamma.

$f_Y(y)=\frac{\tilde\beta^\alpha e^{-\tilde\beta/y}}{\Gamma(\alpha)y^{\alpha+1}}\sim\text{IGamma}(\alpha,1/\beta)$
$\square$

# 3.28

## b

$X\sim\text{Beta}(\alpha,\beta)$

$f(x)=\frac{x^{\alpha-1}(1-x)^{\beta-1}}{B(\alpha,\beta)}$

$f_X(x)=\frac{1}{B(\alpha,\beta)}e^{(\alpha-1)\ln(x)(\beta-1)\ln(1-x)}$

## d

$X\sim\text{Poisson}(\lambda)$
$P(X=x)=\frac{e^{-\lambda}\lambda^x}{x!}$

$P(X=x)=\frac{1}{x!}e^{-\lambda}e^{x\ln(\lambda)}$
$P(X=x)=\frac{1}{x!}e^{-\lambda}e^{x\ln(\lambda)}$


# 3.33

## b
