---
date created: 2023-11-08 11:45
---

# 4.2

## a

$E(ag_1(X,Y)+bg_2(X,Y)+c)=eE(g_1(X,Y))+bE(g_2(X,Y))+c$

---

$E(ag_1(X,Y)+bg_2(X,Y)+c)=\int\limits_{-\infty}^\infty (ag_1(x,y)+bg_2(x,y)+c)f(x,y)$
$=\int\limits_{-\infty}^\infty ag_1(x,y)f(x,y)+bg_2(x,y)f(x,y)+cf(x,y)$
$=\int\limits_{-\infty}^\infty ag_1(x,y)f(x,y)+\int\limits_{-\infty}^\infty bg_2(x,y)f(x,y)+\int\limits_{-\infty}^\infty cf(x,y)$
$=a\int\limits_{-\infty}^\infty g_1(x,y)f(x,y)+b\int\limits_{-\infty}^\infty g_2(x,y)f(x,y)+c\int\limits_{-\infty}^\infty f(x,y)$
$=aE(g_1(X,Y))+bE(g_2(X,Y))+cE(1)$
$=aE(g_1(X,Y))+bE(g_2(X,Y))+c$
$\square$

## b

$g_1(x,y)\ge 0\implies E(g_1(X,Y))\ge 0$



## c

## d

# 4.4

## a

## b

## c

## d

# 4.10

## a

## b
