# 4.22

When
$U=g_1(X,Y)$
$V=g_2(X,Y)$
$X=h_1(U,V)$
$Y=h_2(U,V)$

$f_{U,V}(u,v)=f_{X,Y}(h_1(U,V),h_2(U,V))|J(h)|$

$U=aX+b$
$V=cY+d$
$X=\frac{U-b}{a}$
$Y=\frac{V-d}{c}$

$J=\begin{vmatrix}\frac{1}{a}&0\\0&\frac{1}{c}\end{vmatrix}=\frac{1}{ac}$

$f_{U,V}(u,v)=\frac{1}{ac}f(\frac{u-b}{a},\frac{v-d}{c})$

# 4.23

$f_{X,Y}(x,y)=\frac{\Gamma(\alpha+\beta+\gamma)}{\Gamma(\alpha)\Gamma(\beta)\Gamma(\gamma)}x^{\alpha-1}(1-x)^{\beta-1}y^{\alpha+\beta-1}(1-y)^{\gamma-1}$
$0<x<1,\quad0<y<1$

## a

$U=XY$
$V=Y$
$X=\frac{U}{V}$
$Y=V$

$0<U<V<1$

$f_{U,V}(u,v)=Jf_{X,Y}(\frac{u}{v},v)$

$J=\begin{vmatrix}\frac{1}{V}&\frac{-U}{V^{2}}\\0&1\end{vmatrix}=\frac{1}{V}$

$f_{U,V}(u,v)=\frac{1}{v}\frac{\Gamma(\alpha+\beta+\gamma)}{\Gamma(\alpha)\Gamma(\beta)\Gamma(\gamma)}\left( \frac{u}{v} \right)^{\alpha-1}\left( 1-\left( \frac{u}{v} \right) \right)^{\beta-1}v^{\alpha+\beta-1}(1-v)^{\gamma-1}$
\
$f_U(u)=\int\limits_u^1 \frac{1}{v}\frac{\Gamma(\alpha+\beta+\gamma)}{\Gamma(\alpha)\Gamma(\beta)\Gamma(\gamma)}\left( \frac{u}{v} \right)^{\alpha-1}\left( 1-\left( \frac{u}{v} \right) \right)^{\beta-1}v^{\alpha+\beta-1}(1-v)^{\gamma-1}~dv$
$f_U(u)=\int\limits_u^1 v^{-1}\frac{\Gamma(\alpha+\beta+\gamma)}{\Gamma(\alpha)\Gamma(\beta)\Gamma(\gamma)}u^{\alpha-1}v^{1-\alpha}\left( \frac{v-u}{v} \right)^{\beta-1}v^{\alpha+\beta-1}(1-v)^{\gamma-1}~dv$
$f_U(u)=\frac{\Gamma(\alpha+\beta+\gamma)}{\Gamma(\alpha)\Gamma(\beta)\Gamma(\gamma)}u^{\alpha-1}\int\limits_u^1 \left( \frac{v-u}{v} \right)^{\beta-1}v^{\beta-1}(1-v)^{\gamma-1}~dv$
$f_U(u)=\frac{\Gamma(\alpha+\beta+\gamma)}{\Gamma(\alpha)\Gamma(\beta)\Gamma(\gamma)}u^{\alpha-1}\int\limits_u^1 \left(v-u\right)^{\beta-1}(1-v)^{\gamma-1}~dv$

$y=\frac{1-v}{1-u}\quad dy=\frac{-dv}{1-u}$

$f_U(u)=\frac{\Gamma(\alpha+\beta+\gamma)}{\Gamma(\alpha)\Gamma(\beta)\Gamma(\gamma)}u^{\alpha-1}(1-u)^{\beta-1}(1-u)^{\gamma-1}(1-u)\int\limits_u^1 \left(1-y\right)^{\beta-1}(y)^{\gamma-1}~dv$
$f_U(u)=\frac{\Gamma(\alpha+\beta+\gamma)}{\Gamma(\alpha)\Gamma(\beta+\gamma)}u^{\alpha-1}(1-u)^{\beta+\gamma-1}$

$\rho=\beta+\gamma$

$f_U(u)=\frac{\Gamma(\alpha+\rho)}{\Gamma(\alpha)\Gamma(\rho)}u^{\alpha-1}(1-u)^{\rho-1}$

$\sim\text{Beta}(\alpha,\rho)=\text{Beta}(\alpha,\beta+\gamma)$

## b

$U=XY$
$V=\frac{X}{Y}$
$X=\sqrt{UV}$
$Y=\sqrt{\frac{U}{V}}$

$U<V<\frac{1}{U}\quad0<U<1$

$f_{U,V}(u,v)=Jf_{X,Y}\left( \sqrt{UV},\sqrt{\frac{U}{V}} \right)$

$J=\begin{vmatrix}\frac{V}{2\sqrt{UV}}& \frac{U}{2\sqrt{UV}}\\ \frac{1}{2V\sqrt{\frac{U}{V}}}& \frac{-U}{2V^2\sqrt{\frac{U}{V}}}\end{vmatrix}=\frac{-1}{2V}$

$f_{U,V}(u,v)=\frac{1}{2V}\frac{\Gamma(\alpha+\beta+\gamma)}{\Gamma(\alpha)\Gamma(\beta)\Gamma(\gamma)}\sqrt{UV}^{\alpha-1}(1-\sqrt{UV})^{\beta-1}\sqrt{\frac{U}{V}}^{\alpha+\beta-1}(1-\sqrt{\frac{U}{V}})^{\gamma-1}$
$f_{U}(u)=\int\limits_u^{1/u}\frac{1}{2V}\frac{\Gamma(\alpha+\beta+\gamma)}{\Gamma(\alpha)\Gamma(\beta)\Gamma(\gamma)}\sqrt{UV}^{\alpha-1}(1-\sqrt{UV})^{\beta-1}\sqrt{\frac{U}{V}}^{\alpha+\beta-1}(1-\sqrt{\frac{U}{V}})^{\gamma-1}~dv$
$f_{U}(u)=\int\limits_u^{1/u}\frac{\sqrt U}{2V^{3/2}}\frac{\Gamma(\alpha+\beta+\gamma)}{\Gamma(\alpha)\Gamma(\beta)\Gamma(\gamma)}(\sqrt{\frac{U}{V}}\sqrt{UV})^{\alpha-1}(\sqrt{\frac{U}{V}}(1-\sqrt{UV}))^{\beta-1}(1-\sqrt{\frac{U}{V}})^{\gamma-1}~dv$
$f_{U}(u)=\int\limits_u^{1/u}\frac{\sqrt U}{2V^{3/2}}\frac{\Gamma(\alpha+\beta+\gamma)}{\Gamma(\alpha)\Gamma(\beta)\Gamma(\gamma)}U^{\alpha-1}(\sqrt{\frac{U}{V}}-U)^{\beta-1}(1-\sqrt{\frac{U}{V}})^{\gamma-1}~dv$
$f_{U}(u)=\int\limits_u^{1/u}\frac{\sqrt U}{2V^{3/2}}\frac{\Gamma(\alpha+\beta+\gamma)}{\Gamma(\alpha)\Gamma(\beta)\Gamma(\gamma)}U^{\alpha-1}(1-U)^{\beta+\gamma-2}\left( \frac{\sqrt{\frac{U}{V}}-U}{1-U}\right)^{\beta-1}\left( \frac{1-\sqrt{\frac{U}{V}}}{1-U} \right)^{\gamma-1}~dv$

$Z=\frac{\sqrt{\frac{U}{V}}-U}{1-U}$
$dZ=\frac{\sqrt U}{1-U}\frac{-1}{2V^{3/2}}$

$f_{U}(u)=\int\limits_0^{1}\frac{\Gamma(\alpha+\beta+\gamma)}{\Gamma(\alpha)\Gamma(\beta)\Gamma(\gamma)}U^{\alpha-1}(1-U)^{\beta+\gamma-1}\left( Z\right)^{\beta-1}\left( 1-Z \right)^{\gamma-1}~dz$
$f_{U}(u)=\frac{\Gamma(\alpha+\beta+\gamma)}{\Gamma(\alpha)\Gamma(\beta+\gamma)}U^{\alpha-1}(1-U)^{\beta+\gamma-1}\int\limits_0^{1} \frac{\Gamma(\beta+\gamma)}{\Gamma(\beta)\Gamma(\gamma)}\left( Z\right)^{\beta-1}\left( 1-Z \right)^{\gamma-1}~dz$
$f_{U}(u)=\frac{\Gamma(\alpha+\beta+\gamma)}{\Gamma(\alpha)\Gamma(\beta+\gamma)}U^{\alpha-1}(1-U)^{\beta+\gamma-1}$

$U\sim\text{Beta}(\alpha,\beta+\gamma)$

# 4.24

$X\sim\text{Gamma}(r,1)$
$Y\sim\text{Gamma}(s,1)$

$Z_1=X+Y\quad Z_2=\frac{X}{X+Y}$
$X=Z_1Z_2$
$Y=Z_1-Z_1Z_2$

$0<Z_1$
$0<Z_2<1$

$J=\begin{vmatrix}Z_2&Z_1\\1-Z_2&-Z_1\end{vmatrix}=-Z_1$

$f_{X,Y}(x,y)=\frac{x^{r-1}e^{-x}}{\Gamma(r)}\frac{y^{s-1}e^{-y}}{\Gamma(s)}$

$f_{Z_1,Z_2}(z_1,z_2)=\frac{(z_1z_2)^{r-1}e^{-z_1z_2}}{\Gamma(r)}\frac{(z_1-z_1z_2)^{s-1}e^{-z_1+z_1z_2}}{\Gamma(s)}z_1$
$f_{Z_1,Z_2}(z_1,z_2)=\frac{1}{\Gamma(r)\Gamma(s)}z_1^{r+s-1}e^{-z_1}z_2^{r-1}(1-z_2)^{s-1}$
$f_{Z_1,Z_2}(z_1,z_2)=\frac{1}{\Gamma(r+s)}z_1^{r+s-1}e^{-z_1}\frac{\Gamma(r+s)}{\Gamma(r)\Gamma(s)}z_2^{r-1}(1-z_2)^{s-1}$

# 4.32
## a